CacheNew.v
@@ -14,9 +14,9 @@ Module Type Stuff (dt: DataTypes) (ch: ChannelPerAddr dt).
     Record CommonBehavior :=
       {
         change: forall {t a}, st a (S t) <> st a t -> (exists m, mark mch src dst a t m) \/
-                                                      (exists m, proc mch dst src a t m);
+                                                      (exists m, recv mch dst src a t m);
         sendmChange: forall {t a m}, mark mch src dst a t m -> st a (S t) = to m;
-        procmChange: forall {t a m}, proc mch dst src a t m -> st a (S t) = to m;
+        recvmChange: forall {t a m}, recv mch dst src a t m -> st a (S t) = to m;
         sendrImpSt: forall {t a r}, mark rch src dst a t r -> toRSComp (to r) (st a t);
         sendrImpNoSendr: forall {a t1 t2 r1 r2},
                            t1 < t2 -> mark rch src dst a t1 r1 ->
@@ -24,8 +24,8 @@ Module Type Stuff (dt: DataTypes) (ch: ChannelPerAddr dt).
                            exists t', t1 < t' <= t2 /\ ~ toRSComp (to r1) (st a t');
         sendmFrom: forall {t a m}, mark mch src dst a t m -> from m = st a t;
         sendrFrom: forall {t a r}, mark rch src dst a t r -> from r = st a t;
-        noSendmProcm: forall {t a m}, mark mch src dst a t m ->
-                                      forall {m'}, proc mch dst src a t m' -> False;
+        noSendmRecvm: forall {t a m}, mark mch src dst a t m ->
+                                      forall {m'}, recv mch dst src a t m' -> False;
         noSendmSendr: forall {t a m}, mark mch src dst a t m ->
                                       forall {r}, mark rch src dst a t r -> False
       }.
@@ -33,7 +33,7 @@ Module Type Stuff (dt: DataTypes) (ch: ChannelPerAddr dt).
     Lemma nochange': forall {a t t'},
                        (forall tn, t <= tn < t + t' ->
                                    (forall m, ~ mark mch src dst a tn m) /\
-                                   (forall m, ~ proc mch dst src a tn m)) ->
+                                   (forall m, ~ recv mch dst src a tn m)) ->
                        st a t = st a (t + t').
     Proof.
       intros a t t'.
@@ -42,13 +42,13 @@ Module Type Stuff (dt: DataTypes) (ch: ChannelPerAddr dt).
       firstorder.
       intros noChange.
       assert (help: forall tn, t <= tn < t + t' -> (forall m, ~ mark mch src dst a tn m) /\
-        (forall m, ~ proc mch dst src a tn m)) by (
+        (forall m, ~ recv mch dst src a tn m)) by (
           intros tn comp;
             assert (comp2: t <= tn < t + S t') by omega;
               firstorder).
       assert (stTEqstT': st a t = st a (t + t')) by firstorder.
       assert (nothing: (forall m, ~ mark mch src dst a (t + t') m) /\
-        forall m, ~ proc mch dst src a (t + t') m) by
+        forall m, ~ recv mch dst src a (t + t') m) by
       (assert (t <= t + t' < t + S t'); firstorder).
       rewrite stTEqstT'.
       assert (two: st a (t + S t') = st a (t + t') \/ st a (t + S t') <> st a (t + t')) by decide equality.
@@ -61,7 +61,7 @@ Module Type Stuff (dt: DataTypes) (ch: ChannelPerAddr dt).
     Qed.
 
     Lemma noChange: forall {a t t'}, t < t' -> (forall tn, t <= tn < t' ->
-      (forall m, ~ mark mch src dst a tn m) /\ (forall m, ~ proc mch dst src a tn m)) -> st a t = st a t'.
+      (forall m, ~ mark mch src dst a tn m) /\ (forall m, ~ recv mch dst src a tn m)) -> st a t = st a t'.
     Proof.
       intros a t t' tLtT'.
       remember (t' - t) as td.
@@ -71,7 +71,7 @@ Module Type Stuff (dt: DataTypes) (ch: ChannelPerAddr dt).
     Qed.
 
     Lemma noChange2: forall {a t t'}, t <= t' -> (forall tn, t <= tn < t' ->
-      (forall m, ~ mark mch src dst a tn m) /\ (forall m, ~ proc mch dst src a tn m)) -> st a t = st a t'.
+      (forall m, ~ mark mch src dst a tn m) /\ (forall m, ~ recv mch dst src a tn m)) -> st a t = st a t'.
     Proof.
       intros a t t' tLeT'.
       assert (opts: t = t' \/ t < t') by omega.
@@ -90,30 +90,30 @@ Module Type Stuff (dt: DataTypes) (ch: ChannelPerAddr dt).
     Axiom voluntary:
       forall {a t r}, mark rch c p a t r -> forall {t' m}, t' > t -> mark mch c p a t' m ->
         (forall {tm}, t < tm <= t' -> state c a tm < to r) ->
-        exists r1, proc rch p c a t' r1 /\ state c a t' > to r1.
+        exists r1, recv rch p c a t' r1 /\ state c a t' > to r1.
 
-(*    Axiom procrSendm: forall {r}, proc rch p c a t r -> state c a t > to r -> exists {m}, mark mch c p a t m.*)
+(*    Axiom recvrSendm: forall {r}, recv rch p c a t r -> state c a t > to r -> exists {m}, mark mch c p a t m.*)
 
     Axiom dt: @CommonBehavior (dir p c) lt p c.
     Section ForT.
       Context {a: Addr} {t: Time}.
 
-      Axiom sendmImpProcr: forall {m}, mark mch p c a t m -> exists r, proc rch c p a t r.
+      Axiom sendmImpRecvr: forall {m}, mark mch p c a t m -> exists r, recv rch c p a t r.
 
-      Axiom sendmImpProcrGe: forall {m}, mark mch p c a t m ->
-                                         forall {r}, proc rch c p a t r -> to m >= to r.
+      Axiom sendmImpRecvrGe: forall {m}, mark mch p c a t m ->
+                                         forall {r}, recv rch c p a t r -> to m >= to r.
 
-      Axiom procrCond: forall {r}, proc rch c p a t r -> from r >= dir p c a t.
+      Axiom recvrCond: forall {r}, recv rch c p a t r -> from r >= dir p c a t.
 
-      Axiom procmCond: forall {m}, proc mch c p a t m -> from m = dir p c a t.
+      Axiom recvmCond: forall {m}, recv mch c p a t m -> from m = dir p c a t.
 
       Axiom sendrImpNoSendm: 
         forall {t1 t2 r1 m2},
           t1 < t2 -> mark rch p c a t1 r1 ->
           mark mch p c a t2 m2 ->
-          exists t', t1 < t' < t2 /\ exists m, proc mch c p a t' m /\ to m <= to r1.
+          exists t', t1 < t' < t2 /\ exists m, recv mch c p a t' m /\ to m <= to r1.
 
-      (*    Axiom procrImpSendm: forall {r}, proc rch c p a t r -> exists m, mark mch p c a t m /\ to m >= to r.*)
+      (*    Axiom recvrImpSendm: forall {r}, recv rch c p a t r -> exists m, mark mch p c a t m /\ to m >= to r.*)
     End ForT.
 
     Axiom init: forall {a}, dir p c a 0 = state c a 0.
@@ -121,8 +121,8 @@ Module Type Stuff (dt: DataTypes) (ch: ChannelPerAddr dt).
     Definition twoEqPRespFalse :=
       forall a t t1 m1, t1 <= t -> mark mch p c a t1 m1 ->
                         forall t2 m2, t2 <= t -> mark mch p c a t2 m2 ->
-                                      (forall t3, t3 <= t -> ~ proc mch p c a t3 m1) ->
-                                      (forall {t4}, t4 <= t -> ~ proc mch p c a t4 m2) ->
+                                      (forall t3, t3 <= t -> ~ recv mch p c a t3 m1) ->
+                                      (forall {t4}, t4 <= t -> ~ recv mch p c a t4 m2) ->
                                       t1 = t2.
 
     Definition twoPReqEqNeedsPResp :=
@@ -130,8 +130,8 @@ Module Type Stuff (dt: DataTypes) (ch: ChannelPerAddr dt).
         t1 <= t -> mark rch p c a t1 r1 ->
         forall t2 r2,
           t2 <= t -> mark rch p c a t2 r2 ->
-          (forall t3, t3 <= t -> ~ proc rch p c a t3 r1) ->
-          (forall t4, t4 <= t -> ~ proc rch p c a t4 r2) -> t1 < t2 ->
+          (forall t3, t3 <= t -> ~ recv rch p c a t3 r1) ->
+          (forall t4, t4 <= t -> ~ recv rch p c a t4 r2) -> t1 < t2 ->
           to r1 <= to r2 -> exists tm, t1 < tm < t2 /\ exists m, mark mch p c a tm m.
 
     Section ForA.
@@ -141,16 +141,16 @@ Module Type Stuff (dt: DataTypes) (ch: ChannelPerAddr dt).
                       forall {t1 t2 t3},
                       forall {m},
                         mark mch p c a t1 m ->
-                        forall {r}, mark rch p c a t2 r -> proc rch p c a t3 r -> t1 <= t2 ->
-                                    exists t4, t4 < t3 /\ proc mch p c a t4 m.
+                        forall {r}, mark rch p c a t2 r -> recv rch p c a t3 r -> t1 <= t2 ->
+                                    exists t4, t4 < t3 /\ recv mch p c a t4 m.
 
       Axiom pReqResp: twoEqPRespFalse ->
                       twoPReqEqNeedsPResp ->
                       forall {t1 t2 t3},
                       forall {r},
                         mark rch p c a t1 r ->
-                        forall {m}, mark mch p c a t2 m -> proc mch p c a t3 m -> t1 <= t2 ->
-                                    exists t4, t4 < t3 /\ proc rch p c a t4 r.
+                        forall {m}, mark mch p c a t2 m -> recv mch p c a t3 m -> t1 <= t2 ->
+                                    exists t4, t4 < t3 /\ recv rch p c a t4 r.
     End ForA.
 
     Axiom classical: forall P, P \/ ~ P.
@@ -168,28 +168,28 @@ Module Final (dt: DataTypes) (ch: ChannelPerAddr dt) (st: Stuff dt ch).
     Definition dt := @st.dt p c.
 
 
-      Lemma whenChildHighProcm: forall {a t},
+      Lemma whenChildHighRecvm: forall {a t},
                                   state c a (S t) > state c a t ->
-                                  exists m, proc mch p c a t m /\ to m = state c a (S t).
+                                  exists m, recv mch p c a t m /\ to m = state c a (S t).
       Proof.
         intros a t sStgst.
         assert (sStnst: state c a (S t) <> state c a t) by omega.
-        pose proof (change st sStnst) as [[m sendmm] | [m procmm] ].
+        pose proof (change st sStnst) as [[m sendmm] | [m recvmm] ].
         pose proof (sendmImpSt sendmm) as stgm.
         pose proof (sendmChange st sendmm) as sStem.
         omega.
         exists m.
         intuition.
-        pose proof (procmChange st procmm) as sStem.
+        pose proof (recvmChange st recvmm) as sStem.
         intuition.
       Qed.
 
       Lemma whenChildHigh': forall {a t t'}, state c a (S (t' + t)) > state c a t ->
-                                           exists t'', t'' <= t' /\ exists m, proc mch p c a (t'' + t) m /\ to m >= state c a (S (t' + t)).
+                                           exists t'', t'' <= t' /\ exists m, recv mch p c a (t'' + t) m /\ to m >= state c a (S (t' + t)).
       Proof.
         intros a t t' sSt'tgst.
         induction t'.
-        pose proof (whenChildHighProcm sSt'tgst) as [m [procmm mesSt]].
+        pose proof (whenChildHighRecvm sSt'tgst) as [m [recvmm mesSt]].
         exists 0.
         assert (temp: 0 + t = t) by omega.
         rewrite temp in *; clear temp.
@@ -199,7 +199,7 @@ Module Final (dt: DataTypes) (ch: ChannelPerAddr dt) (st: Stuff dt ch).
         pose proof (lt_eq_lt_dec (state c a (S (S t' + t))) (state c a (S (t' + t)))) as [[lt | eq] | gt'].
         assert (gt: state c a (S (t' + t)) > state c a t) by omega.
         specialize (IHt' gt).
-        destruct IHt' as [t'' [le [m [procmm mgesSt't]]]].
+        destruct IHt' as [t'' [le [m [recvmm mgesSt't]]]].
         assert (t''leSt': t'' <= S t') by omega.
         assert (mgesSSt't: to m >= state c a (S (S t' + t))) by omega.
         exists t''.
@@ -212,7 +212,7 @@ Module Final (dt: DataTypes) (ch: ChannelPerAddr dt) (st: Stuff dt ch).
         exists t''.
         intuition.
         assert (gt: state c a (S (S t' + t)) > state c a (S (t' + t))) by omega; clear gt'.
-        pose proof (whenChildHighProcm gt) as [m [procmm mesSt]].
+        pose proof (whenChildHighRecvm gt) as [m [recvmm mesSt]].
         exists (S t').
         intuition.
         exists m.
@@ -220,7 +220,7 @@ Module Final (dt: DataTypes) (ch: ChannelPerAddr dt) (st: Stuff dt ch).
       Qed.
 
       Lemma whenChildHigh: forall {a t t'}, t' > t -> state c a t' > state c a t ->
-                                          exists t'', t <= t'' < t' /\ exists m, proc mch p c a t'' m /\ to m >= state c a t'.
+                                          exists t'', t <= t'' < t' /\ exists m, recv mch p c a t'' m /\ to m >= state c a t'.
       Proof.
         intros a t tPlust'.
         intros diff.
@@ -236,7 +236,7 @@ Module Final (dt: DataTypes) (ch: ChannelPerAddr dt) (st: Stuff dt ch).
       Qed.
 
       Lemma whenChildHighConv: forall {a t t'}, t' >= t ->
-                                              (~ exists t'', t <= t'' < t' /\ exists m, proc mch p c a t'' m /\ to m >= state c a t') ->
+                                              (~ exists t'', t <= t'' < t' /\ exists m, recv mch p c a t'' m /\ to m >= state c a t') ->
                                               state c a t' <= state c a t.
       Proof.
         intros a t t' t'GeT notE.
@@ -248,13 +248,13 @@ Module Final (dt: DataTypes) (ch: ChannelPerAddr dt) (st: Stuff dt ch).
         omega.
       Qed.
 
-    Lemma dirProcImpLow: forall {a t m}, proc mch c p a t m -> dir p c a t > dir p c a (S t).
+    Lemma dirRecvImpLow: forall {a t m}, recv mch c p a t m -> dir p c a t > dir p c a (S t).
     Proof.
-      intros a t m procm.
-      pose proof (procImpMark procm) as [t' [t'LeT sendm]].
-      pose proof (procmChange dt procm) as sth.
+      intros a t m recvm.
+      pose proof (recvImpMark recvm) as [t' [t'LeT sendm]].
+      pose proof (recvmChange dt recvm) as sth.
       pose proof (sendmImpSt sendm) as sth2.
-      pose proof (procmCond procm) as sth3.
+      pose proof (recvmCond recvm) as sth3.
       pose proof (sendmFrom st sendm) as sth4.
       omega.
     Qed.
@@ -274,10 +274,10 @@ Module Final (dt: DataTypes) (ch: ChannelPerAddr dt) (st: Stuff dt ch).
       assert (gt: dir p c a (S (t' + t)) > dir p c a (t' + t)) by (assert (eq: S t' + t = S (t' + t)) by omega;
                                                                    rewrite eq in *; omega).
       assert (nestuff: dir p c a (S (t' + t)) <> dir p c a (t' + t)) by omega.
-      pose proof (change dt nestuff) as [sendm | procm].
+      pose proof (change dt nestuff) as [sendm | recvm].
       firstorder.
-      destruct procm as [x procstuff].
-      pose proof (dirProcImpLow procstuff) as contra.
+      destruct recvm as [x recvstuff].
+      pose proof (dirRecvImpLow recvstuff) as contra.
       omega.
     Qed.
 
@@ -302,7 +302,7 @@ Module Final (dt: DataTypes) (ch: ChannelPerAddr dt) (st: Stuff dt ch).
                       forall {td},
                         ~ (exists tn, t <= tn < t + td /\
                                       ((exists m, mark mch p c a tn m) \/
-                                       (exists m, proc mch c p a tn m /\ to m <= x))) ->
+                                       (exists m, recv mch c p a tn m /\ to m <= x))) ->
                         dir p c a (t + td) > x.
     Proof.
       intros a t x cond.
@@ -313,7 +313,7 @@ Module Final (dt: DataTypes) (ch: ChannelPerAddr dt) (st: Stuff dt ch).
       intuition.
       intros nothing.
       assert (contra: ~ exists tn, t <= tn < t + td /\ ((exists m, mark mch p c a tn m) \/
-                                                        (exists m, proc mch c p a tn m /\ to m <= x))) by (unfold not; intros [tn [cond3 rest]];
+                                                        (exists m, recv mch c p a tn m /\ to m <= x))) by (unfold not; intros [tn [cond3 rest]];
                                                                                                            assert (cond2: t <= tn < t + S td) by omega;
                                                                                                            generalize nothing cond2 rest; clear; firstorder).
       specialize (IHtd contra).
@@ -327,12 +327,12 @@ Module Final (dt: DataTypes) (ch: ChannelPerAddr dt) (st: Stuff dt ch).
       rewrite eq in *.
       specialize (stUnEq hard).
       assert (pre: t <= t + td < S (t + td)) by omega.
-      destruct stUnEq as [[m sendm]|[m procm]].
+      destruct stUnEq as [[m sendm]|[m recvm]].
       firstorder.
       assert (opts: to m <= x \/ to m > x) by omega.
       destruct opts as [toMLeX | toMGtX].
       firstorder.
-      pose proof (procmChange dt procm).
+      pose proof (recvmChange dt recvm).
       omega.
     Qed.
 
@@ -342,7 +342,7 @@ Module Final (dt: DataTypes) (ch: ChannelPerAddr dt) (st: Stuff dt ch).
                               t <= t1 ->
                               ~ (exists tn, t <= tn < t1 /\
                                             ((exists m, mark mch p c a tn m) \/
-                                             (exists m, proc mch c p a tn m /\ to m <= x))) ->
+                                             (exists m, recv mch c p a tn m /\ to m <= x))) ->
                               dir p c a (t1) > x.
     Proof.
       intros a t x dirx t1 tLeT1 contra.
@@ -359,27 +359,27 @@ Module Final (dt: DataTypes) (ch: ChannelPerAddr dt) (st: Stuff dt ch).
         tc <= t -> tp <= t -> 
         forall {r m}, mark rch c p a tc r ->
                       mark mch p c a tp m ->
-                      (forall tc', tc' < tc -> ~ proc mch p c a tc' m) ->
-                      (forall tp', tp' <= tp -> ~ proc rch c p a tp' r) -> False.
+                      (forall tc', tc' < tc -> ~ recv mch p c a tc' m) ->
+                      (forall tp', tp' <= tp -> ~ recv rch c p a tp' r) -> False.
     Proof.
       intros a t.
       induction t.
-      intros tc tp tcLeT tpLeT r m rsendr msendm mprocNo rprocNo.
+      intros tc tp tcLeT tpLeT r m rsendr msendm mrecvNo rrecvNo.
       assert (tc0: tc = 0) by omega; clear tcLeT.
       assert (tp0: tp = 0) by omega; clear tpLeT.
       rewrite tc0 in *; rewrite tp0 in *; clear tc0 tp0.
-      pose proof (sendmImpProcr msendm) as [r' rprocr'].
-      pose proof (procImpMark rprocr') as [t' [t'Le0 rsendr']].
+      pose proof (sendmImpRecvr msendm) as [r' rrecvr'].
+      pose proof (recvImpMark rrecvr') as [t' [t'Le0 rsendr']].
       assert (t'0: t' = 0) by omega; clear t'Le0.
       rewrite t'0 in rsendr'; clear t'0.
       pose proof (uniqMark1 rsendr rsendr') as rEqr'.
       rewrite <- rEqr' in *; clear rEqr'.
       assert (zero: 0 <= 0) by omega.
       firstorder.
-      intros tc tp tcLeST tpLeST r m rsendr msendm mprocNo rprocNo.
+      intros tc tp tcLeST tpLeST r m rsendr msendm mrecvNo rrecvNo.
 
-      pose proof (sendmImpProcr msendm) as [r' rprocr'].
-      pose proof (procImpMark rprocr') as [t' [t'LeSt rsendr']].
+      pose proof (sendmImpRecvr msendm) as [r' rrecvr'].
+      pose proof (recvImpMark rrecvr') as [t' [t'LeSt rsendr']].
 
       assert (diff: t' = tc \/ t' > tc \/ t' < tc) by omega.
       destruct diff as [eq | [t'GtTc | tcGtT']].
@@ -394,55 +394,55 @@ Module Final (dt: DataTypes) (ch: ChannelPerAddr dt) (st: Stuff dt ch).
       pose proof (sendrImpSt st rsendr) as toGtt.
       assert (tcLtT'': state c a tc < state c a t'') by omega.
       assert (t''GtTc: t'' > tc) by omega.
-      pose proof (whenChildHigh t''GtTc tcLtT'') as [t''' [[tcLeT''' t'''LtT''] [m' [mprocm' _]]]].
-      pose proof (procImpMark mprocm') as [td [tdLeT''' msendm']].
+      pose proof (whenChildHigh t''GtTc tcLtT'') as [t''' [[tcLeT''' t'''LtT''] [m' [mrecvm' _]]]].
+      pose proof (recvImpMark mrecvm') as [td [tdLeT''' msendm']].
       assert (tdLet: td <= t) by omega.
-      assert (noProc: forall tc', tc' < tc -> ~ proc mch p c a tc' m') by (
-                                                                           unfold not; intros tc' tc'LtTc mprocm'Tc';
-                                                                           pose proof (uniqProc2 mprocm' mprocm'Tc') as tc'EqT''; omega).
-      assert (noProc': forall tp', tp' <= td -> ~ proc rch c p a tp' r) by (
+      assert (noRecv: forall tc', tc' < tc -> ~ recv mch p c a tc' m') by (
+                                                                           unfold not; intros tc' tc'LtTc mrecvm'Tc';
+                                                                           pose proof (uniqRecv2 mrecvm' mrecvm'Tc') as tc'EqT''; omega).
+      assert (noRecv': forall tp', tp' <= td -> ~ recv rch c p a tp' r) by (
                                                                             unfold not; intros tp' tp'LeTd;
                                                                             assert (tp'LeTp: tp' <= tp) by omega;
                                                                             firstorder).
       assert (tcLeT: tc <= t) by omega.
-      apply (IHt tc td tcLeT tdLet r m' rsendr msendm' noProc noProc').
+      apply (IHt tc td tcLeT tdLet r m' rsendr msendm' noRecv noRecv').
 
       pose proof (sendrImpNoSendr st tcGtT' rsendr' rsendr) as [tmur [cond neg]].
       assert (toRLeS: to r' <= state c a tmur) by omega.
       pose proof (sendrImpSt st rsendr') as toGtt.
       assert (stt'LtstTc: state c a t' < state c a tmur) by omega.
       assert (tmurGtT': tmur > t') by omega.
-      pose proof (whenChildHigh tmurGtT' stt'LtstTc) as [t'' [[tcLeT'' t''LtT'] [m' [mprocm' _]]]].
-      pose proof (procImpMark mprocm') as [td [tdLeT'' msendm']].
+      pose proof (whenChildHigh tmurGtT' stt'LtstTc) as [t'' [[tcLeT'' t''LtT'] [m' [mrecvm' _]]]].
+      pose proof (recvImpMark mrecvm') as [td [tdLeT'' msendm']].
       assert (tdLet: td <= t) by omega.
-      assert (noProc: forall tc', tc' < t' -> ~ proc mch p c a tc' m') by (
-                                                                           unfold not; intros tc' tc'LtTc mprocm'Tc';
-                                                                           pose proof (uniqProc2 mprocm' mprocm'Tc') as tc'EqT''; omega).
+      assert (noRecv: forall tc', tc' < t' -> ~ recv mch p c a tc' m') by (
+                                                                           unfold not; intros tc' tc'LtTc mrecvm'Tc';
+                                                                           pose proof (uniqRecv2 mrecvm' mrecvm'Tc') as tc'EqT''; omega).
       assert (opts: td = tp \/ td < tp \/ td > tp) by omega.
-      destruct opts as [tprocTp | [tdLTp | tdGtTp]].
-      rewrite tprocTp in *.
+      destruct opts as [trecvTp | [tdLTp | tdGtTp]].
+      rewrite trecvTp in *.
       pose proof (uniqMark1 msendm msendm') as mEqm'.
       rewrite <- mEqm' in *.
       assert (t''LtTc: t'' < tc) by omega.
       firstorder.
-      assert (noProc': forall tp', tp' <= td -> ~ proc rch c p a tp' r') by (
-                                                                             unfold not; intros tp' tp'LeTd rprocr'Tp';
-                                                                             pose proof (uniqProc2 rprocr' rprocr'Tp') as tp'EqTp;
+      assert (noRecv': forall tp', tp' <= td -> ~ recv rch c p a tp' r') by (
+                                                                             unfold not; intros tp' tp'LeTd rrecvr'Tp';
+                                                                             pose proof (uniqRecv2 rrecvr' rrecvr'Tp') as tp'EqTp;
                                                                              omega).
       assert (t'LeT: t' <= t) by omega.
-      apply (IHt t' td t'LeT tdLet r' m' rsendr' msendm' noProc noProc').
-      pose proof (sendmImpProcr msendm') as [r'' rprocr''].
-      pose proof (procImpMark rprocr'') as [ts [tsLeTd rsendr'']].
+      apply (IHt t' td t'LeT tdLet r' m' rsendr' msendm' noRecv noRecv').
+      pose proof (sendmImpRecvr msendm') as [r'' rrecvr''].
+      pose proof (recvImpMark rrecvr'') as [ts [tsLeTd rsendr'']].
       assert (tpLeT: tp <= t) by omega.
       assert (tsLeT: ts <= t) by omega.
-      assert (hyp1: forall tc', tc' < ts -> ~ proc mch p c a tc' m) by (
+      assert (hyp1: forall tc', tc' < ts -> ~ recv mch p c a tc' m) by (
                                                                         intros tc' tc'LtTs;
                                                                         assert (tc'LtTc: tc' < tc) by omega;
                                                                         firstorder).
-      assert (hyp2: forall tp', tp' <= tp -> ~ proc rch c p a tp' r'') by (
-                                                                           unfold not; intros tp' tpLeTp rprocr''Tp';
-                                                                           pose proof (uniqProc2 rprocr'' rprocr''Tp') as tprocTp';
-                                                                           rewrite <- tprocTp' in *;
+      assert (hyp2: forall tp', tp' <= tp -> ~ recv rch c p a tp' r'') by (
+                                                                           unfold not; intros tp' tpLeTp rrecvr''Tp';
+                                                                           pose proof (uniqRecv2 rrecvr'' rrecvr''Tp') as trecvTp';
+                                                                           rewrite <- trecvTp' in *;
                                                                              firstorder).
       apply (IHt ts tp tsLeT tpLeT r'' m rsendr'' msendm hyp1 hyp2).
     Qed.
@@ -450,8 +450,8 @@ Module Final (dt: DataTypes) (ch: ChannelPerAddr dt) (st: Stuff dt ch).
     Lemma cReqPRespCross:
       forall {a tc tp r m},
         mark rch c p a tc r ->
-        mark mch p c a tp m -> (forall tc', tc' < tc -> ~ proc mch p c a tc' m) ->
-        (forall tp', tp' <= tp -> ~ proc rch c p a tp' r) -> False.
+        mark mch p c a tp m -> (forall tc', tc' < tc -> ~ recv mch p c a tc' m) ->
+        (forall tp', tp' <= tp -> ~ recv rch c p a tp' r) -> False.
     Proof.
       intros a tc tp.
       assert (tcLeT: tc <= tc + tp) by omega.
@@ -463,23 +463,23 @@ Module Final (dt: DataTypes) (ch: ChannelPerAddr dt) (st: Stuff dt ch).
                        ts1 < ts2 ->
                        mark mch p c a ts1 m1 ->
                        mark mch p c a ts2 m2 ->
-                       proc mch p c a tr2 m2 ->
-                       exists tr1, tr1 < tr2 /\ proc mch p c a tr1 m1.
-      intros a ts1 ts2 tr2 m1 m2 ts1_lt_ts2 markm1 markm2 procm2.
-      pose proof (sendmImpProcr markm2) as [r2 procr2].
-      assert (noRecvr: forall tp', tp' <= ts1 -> ~ proc rch c p a tp' r2)
+                       recv mch p c a tr2 m2 ->
+                       exists tr1, tr1 < tr2 /\ recv mch p c a tr1 m1.
+      intros a ts1 ts2 tr2 m1 m2 ts1_lt_ts2 markm1 markm2 recvm2.
+      pose proof (sendmImpRecvr markm2) as [r2 recvr2].
+      assert (noRecvr: forall tp', tp' <= ts1 -> ~ recv rch c p a tp' r2)
         by (
-            unfold not; intros tp' tp'_le_ts1 proc'r2;
-            pose proof (uniqProc2 procr2 proc'r2);
+            unfold not; intros tp' tp'_le_ts1 recv'r2;
+            pose proof (uniqRecv2 recvr2 recv'r2);
             omega).
-      pose proof (procImpMark procr2) as [tsr2 [tsr2_le_ts2 markr2]].
-      destruct (classical (exists tr1, tr1 < tr2 /\ proc mch p c a tr1 m1)) as [easy|hard].
+      pose proof (recvImpMark recvr2) as [tsr2 [tsr2_le_ts2 markr2]].
+      destruct (classical (exists tr1, tr1 < tr2 /\ recv mch p c a tr1 m1)) as [easy|hard].
       assumption.
-      assert (noRecvm1: forall tr1, tr1 < tr2 -> ~ proc mch p c a tr1 m1) by firstorder.
+      assert (noRecvm1: forall tr1, tr1 < tr2 -> ~ recv mch p c a tr1 m1) by firstorder.
       clear hard.
-      pose proof (procImpMarkBefore procm2 markm2) as ts2_le_tr2.
+      pose proof (recvImpMarkBefore recvm2 markm2) as ts2_le_tr2.
       assert (tsr2_le_tr2: tsr2 <= tr2) by omega.
-      assert (noRecv'm1: forall tc', tc' < tsr2 -> ~ proc mch p c a tc' m1) by
+      assert (noRecv'm1: forall tc', tc' < tsr2 -> ~ recv mch p c a tc' m1) by
           (
             intros tc' tc'_lt_tsr2; assert (tc'_lt_tr2: tc' < tr2) by omega; generalize noRecvm1 tc'_lt_tr2; clear; firstorder).
       pose proof (cReqPRespCross markr2 markm1 noRecv'm1 noRecvr) as [].
@@ -487,92 +487,92 @@ Module Final (dt: DataTypes) (ch: ChannelPerAddr dt) (st: Stuff dt ch).
 
     Lemma noTwoPResp: @twoEqPRespFalse p c.
     Proof.
-      intros a tx t1 m1 t1LeTx sendm1 t2 m2 t2LeTx sendm2 noprocm1 noprocm2.
-      pose proof (sendmImpProcr sendm1) as [r1 procr1].
-      pose proof (sendmImpProcr sendm2) as [r2 procr2].
-      pose proof (procImpMark procr1) as [t3 [t3LeT1 sendr1]].
-      pose proof (procImpMark procr2) as [t4 [t4LeT2 sendr2]].
+      intros a tx t1 m1 t1LeTx sendm1 t2 m2 t2LeTx sendm2 norecvm1 norecvm2.
+      pose proof (sendmImpRecvr sendm1) as [r1 recvr1].
+      pose proof (sendmImpRecvr sendm2) as [r2 recvr2].
+      pose proof (recvImpMark recvr1) as [t3 [t3LeT1 sendr1]].
+      pose proof (recvImpMark recvr2) as [t4 [t4LeT2 sendr2]].
       assert (opts: t3 = t4 \/ t3 < t4 \/ t4 < t3) by omega.
       destruct opts as [t3EqT4|[t3LtT4|t4LtT3]].
       rewrite t3EqT4 in *; pose proof (uniqMark1 sendr1 sendr2) as r1EqR2.
-      rewrite r1EqR2 in *; apply (uniqProc2 procr1 procr2).
+      rewrite r1EqR2 in *; apply (uniqRecv2 recvr1 recvr2).
 
-      assert (noProc: ~ exists t, t3 <= t < t4 /\ exists m, proc mch p c a t m) by (
-                                                                                    unfold not; intros [t [cond [m procm]]];
-                                                                                    pose proof (procImpMark procm) as [t5 [t5LeT sendm]];
+      assert (noRecv: ~ exists t, t3 <= t < t4 /\ exists m, recv mch p c a t m) by (
+                                                                                    unfold not; intros [t [cond [m recvm]]];
+                                                                                    pose proof (recvImpMark recvm) as [t5 [t5LeT sendm]];
                                                                                     assert (opts: t5 = t1 \/ t5 < t1 \/ t5 > t1) by omega;
                                                                                     destruct opts as [t5EqT1 | [t5LtT1 | t5GtT1]]; [
                                                                                       rewrite t5EqT1 in *; pose proof (uniqMark1 sendm1 sendm) as m1EqM;
                                                                                       rewrite m1EqM in *; assert (tLeTx: t <= tx) by omega;
-                                                                                      generalize tLeTx noprocm1 procm; clear; firstorder |
-                                                                                      assert (one: forall tc', tc' < t3 -> ~ proc mch p c a tc' m) by (
-                                                                                                                                                       unfold not; intros tc' tc'LtT3 proc'm; pose proof (uniqProc2 procm proc'm) as tEqTc';
+                                                                                      generalize tLeTx norecvm1 recvm; clear; firstorder |
+                                                                                      assert (one: forall tc', tc' < t3 -> ~ recv mch p c a tc' m) by (
+                                                                                                                                                       unfold not; intros tc' tc'LtT3 recv'm; pose proof (uniqRecv2 recvm recv'm) as tEqTc';
                                                                                                                                                        rewrite tEqTc' in *; firstorder);
-                                                                                        assert (two: forall tp', tp' <= t5 -> ~ proc rch c p a tp' r1) by (
-                                                                                                                                                           unfold not; intros tp' tp'LeT1 proc'r1; pose proof (uniqProc2 procr1 proc'r1) as t5EqTp';
+                                                                                        assert (two: forall tp', tp' <= t5 -> ~ recv rch c p a tp' r1) by (
+                                                                                                                                                           unfold not; intros tp' tp'LeT1 recv'r1; pose proof (uniqRecv2 recvr1 recv'r1) as t5EqTp';
                                                                                                                                                            rewrite <- t5EqTp' in *; firstorder);
                                                                                         apply (cReqPRespCross sendr1 sendm one two) |
-                                                                                      pose proof (sendmImpProcr sendm) as [r procr];
-                                                                                        pose proof (procImpMark procr) as [t6 [t6LeT5 sendr]];
-                                                                                        assert (one: forall tc', tc' < t6 -> ~ proc mch p c a tc' m1) by (
-                                                                                                                                                          unfold not; intros tc' tc'LtT6 proc'm1; assert (tc'LeT6: tc' <= tx) by omega;
-                                                                                                                                                          generalize noprocm1 proc'm1 tc'LeT6; clear; firstorder);
-                                                                                        assert (two: forall tp', tp' <= t1 -> ~ proc rch c p a tp' r) by (
-                                                                                                                                                          unfold not; intros tp' tp'LeT1 proc'r; pose proof (uniqProc2 procr proc'r) as t1EqTp';
+                                                                                      pose proof (sendmImpRecvr sendm) as [r recvr];
+                                                                                        pose proof (recvImpMark recvr) as [t6 [t6LeT5 sendr]];
+                                                                                        assert (one: forall tc', tc' < t6 -> ~ recv mch p c a tc' m1) by (
+                                                                                                                                                          unfold not; intros tc' tc'LtT6 recv'm1; assert (tc'LeT6: tc' <= tx) by omega;
+                                                                                                                                                          generalize norecvm1 recv'm1 tc'LeT6; clear; firstorder);
+                                                                                        assert (two: forall tp', tp' <= t1 -> ~ recv rch c p a tp' r) by (
+                                                                                                                                                          unfold not; intros tp' tp'LeT1 recv'r; pose proof (uniqRecv2 recvr recv'r) as t1EqTp';
                                                                                                                                                           rewrite <- t1EqTp' in *; firstorder);
                                                                                         apply (cReqPRespCross sendr sendm1 one two)]).
       assert (t3LeT4: t3 <= t4) by omega.
       pose proof (sendrImpSt st sendr1) as stG.
       pose proof (sendrImpNoSendr st t3LtT4 sendr1 sendr2) as [t5 [t3LtT5LeT4 neg]].
       assert (pos: state c a t5 > state c a t3) by omega.
-      assert (noProc': ~ exists t, t3 <= t < t5 /\ exists m, proc mch p c a t m /\ to m >= state c a t5) by (
-                                                                                                             unfold not; intros [t [cond1 [mg [procmg _]]]];
+      assert (noRecv': ~ exists t, t3 <= t < t5 /\ exists m, recv mch p c a t m /\ to m >= state c a t5) by (
+                                                                                                             unfold not; intros [t [cond1 [mg [recvmg _]]]];
                                                                                                              assert (cond: t3 <= t < t4) by omega;
-                                                                                                             generalize procmg cond noProc; clear; firstorder).
+                                                                                                             generalize recvmg cond noRecv; clear; firstorder).
       assert (t3LeT5: t3 <= t5) by omega.
-      pose proof (whenChildHighConv t3LeT5 noProc') as stContra.
+      pose proof (whenChildHighConv t3LeT5 noRecv') as stContra.
       omega.
 
-      assert (noProc: ~ exists t, t4 <= t < t3 /\ exists m, proc mch p c a t m) by (
-                                                                                    unfold not; intros [t [cond [m procm]]];
-                                                                                    pose proof (procImpMark procm) as [t5 [t5LeT sendm]];
+      assert (noRecv: ~ exists t, t4 <= t < t3 /\ exists m, recv mch p c a t m) by (
+                                                                                    unfold not; intros [t [cond [m recvm]]];
+                                                                                    pose proof (recvImpMark recvm) as [t5 [t5LeT sendm]];
                                                                                     assert (opts: t5 = t2 \/ t5 < t2 \/ t5 > t2) by omega;
                                                                                     destruct opts as [t5EqT1 | [t5LtT1 | t5GtT1]]; [
                                                                                       rewrite t5EqT1 in *; pose proof (uniqMark1 sendm2 sendm) as m1EqM;
                                                                                       rewrite m1EqM in *; assert (tLeTx: t <= tx) by omega;
-                                                                                      generalize tLeTx noprocm2 procm; clear; firstorder |
-                                                                                      assert (one: forall tc', tc' < t4 -> ~ proc mch p c a tc' m) by (
-                                                                                                                                                       unfold not; intros tc' tc'LtT3 proc'm; pose proof (uniqProc2 procm proc'm) as tEqTc';
+                                                                                      generalize tLeTx norecvm2 recvm; clear; firstorder |
+                                                                                      assert (one: forall tc', tc' < t4 -> ~ recv mch p c a tc' m) by (
+                                                                                                                                                       unfold not; intros tc' tc'LtT3 recv'm; pose proof (uniqRecv2 recvm recv'm) as tEqTc';
                                                                                                                                                        rewrite tEqTc' in *; firstorder);
-                                                                                        assert (two: forall tp', tp' <= t5 -> ~ proc rch c p a tp' r2) by (
-                                                                                                                                                           unfold not; intros tp' tp'LeT1 proc'r1; pose proof (uniqProc2 procr2 proc'r1) as t5EqTp';
+                                                                                        assert (two: forall tp', tp' <= t5 -> ~ recv rch c p a tp' r2) by (
+                                                                                                                                                           unfold not; intros tp' tp'LeT1 recv'r1; pose proof (uniqRecv2 recvr2 recv'r1) as t5EqTp';
                                                                                                                                                            rewrite <- t5EqTp' in *; firstorder);
                                                                                         apply (cReqPRespCross sendr2 sendm one two)|
-                                                                                      pose proof (sendmImpProcr sendm) as [r procr];
-                                                                                        pose proof (procImpMark procr) as [t6 [t6LeT5 sendr]];
-                                                                                        assert (one: forall tc', tc' < t6 -> ~ proc mch p c a tc' m2) by (
-                                                                                                                                                          unfold not; intros tc' tc'LtT6 proc'm1; assert (tc'LeT6: tc' <= tx) by omega;
-                                                                                                                                                          generalize noprocm2 proc'm1 tc'LeT6; clear; firstorder);
-                                                                                        assert (two: forall tp', tp' <= t2 -> ~ proc rch c p a tp' r) by (
-                                                                                                                                                          unfold not; intros tp' tp'LeT1 proc'r; pose proof (uniqProc2 procr proc'r) as t1EqTp';
+                                                                                      pose proof (sendmImpRecvr sendm) as [r recvr];
+                                                                                        pose proof (recvImpMark recvr) as [t6 [t6LeT5 sendr]];
+                                                                                        assert (one: forall tc', tc' < t6 -> ~ recv mch p c a tc' m2) by (
+                                                                                                                                                          unfold not; intros tc' tc'LtT6 recv'm1; assert (tc'LeT6: tc' <= tx) by omega;
+                                                                                                                                                          generalize norecvm2 recv'm1 tc'LeT6; clear; firstorder);
+                                                                                        assert (two: forall tp', tp' <= t2 -> ~ recv rch c p a tp' r) by (
+                                                                                                                                                          unfold not; intros tp' tp'LeT1 recv'r; pose proof (uniqRecv2 recvr recv'r) as t1EqTp';
                                                                                                                                                           rewrite <- t1EqTp' in *; firstorder);
                                                                                         apply (cReqPRespCross sendr sendm2 one two)]).
       assert (t3LeT4: t4 <= t3) by omega.
       pose proof (sendrImpSt st sendr2) as stG.
       pose proof (sendrImpNoSendr st t4LtT3 sendr2 sendr1) as [t5 [t3LtT5LeT4 neg]].
       assert (pos: state c a t5 > state c a t4) by omega.
-      assert (noProc': ~ exists t, t4 <= t < t5 /\ exists m, proc mch p c a t m /\ to m >= state c a t5) by (
-                                                                                                             unfold not; intros [t [cond1 [mg [procmg _]]]];
+      assert (noRecv': ~ exists t, t4 <= t < t5 /\ exists m, recv mch p c a t m /\ to m >= state c a t5) by (
+                                                                                                             unfold not; intros [t [cond1 [mg [recvmg _]]]];
                                                                                                              assert (cond: t4 <= t < t3) by omega;
-                                                                                                             generalize procmg cond noProc; clear; firstorder).
+                                                                                                             generalize recvmg cond noRecv; clear; firstorder).
       assert (t3LeT5: t4 <= t5) by omega.
-      pose proof (whenChildHighConv t3LeT5 noProc') as stContra.
+      pose proof (whenChildHighConv t3LeT5 noRecv') as stContra.
       omega.
     Qed.
 
     Lemma noTwoPReqNon: @twoPReqEqNeedsPResp p c.
     Proof.
-      intros a t t1 r1 t1LeT sendr1 t2 r2 t2LeT sendr2 noprocr1 noprocr2 t1LtT2 toR1GeToR2.
+      intros a t t1 r1 t1LeT sendr1 t2 r2 t2LeT sendr2 norecvr1 norecvr2 t1LtT2 toR1GeToR2.
       pose proof (sendrImpSt dt sendr1) as gt1.
       pose proof (sendrImpSt dt sendr2) as gt2.
       pose proof (sendrImpNoSendr dt t1LtT2 sendr1 sendr2) as [t5 [cond dr]].
@@ -587,14 +587,14 @@ Module Final (dt: DataTypes) (ch: ChannelPerAddr dt) (st: Stuff dt ch).
     Lemma mainInd: forall {a t},
                      (forall {to}, to <= t -> state c a to <= dir p c a to) /\
                      (forall {tc tp}, tc <= t -> tp <= t -> forall {mc}, mark mch c p a tc mc ->
-                                                                         forall {mp}, mark mch p c a tp mp -> (forall tc', tc' < tc -> ~ proc mch p c a tc' mp) ->
-                                                                                      (forall tp', tp' < tp -> ~ proc mch c p a tp' mc) -> False) /\
+                                                                         forall {mp}, mark mch p c a tp mp -> (forall tc', tc' < tc -> ~ recv mch p c a tc' mp) ->
+                                                                                      (forall tp', tp' < tp -> ~ recv mch c p a tp' mc) -> False) /\
                      (forall {t1 t2 t3}, t3 <= t -> forall {m}, mark mch c p a t1 m ->
-                                                                forall {r}, mark rch c p a t2 r -> proc rch c p a t3 r -> t1 <= t2 ->
-                                                                            (forall t4, t4 < t3 -> ~ proc mch c p a t4 m) -> False) /\
+                                                                forall {r}, mark rch c p a t2 r -> recv rch c p a t3 r -> t1 <= t2 ->
+                                                                            (forall t4, t4 < t3 -> ~ recv mch c p a t4 m) -> False) /\
                      (forall {t1 t2 t3}, t3 <= t -> forall {m}, mark mch c p a t1 m ->
-                                                                forall {m'}, mark mch c p a t2 m' -> proc mch c p a t3 m' -> t1 < t2 ->
-                                                                             (forall t4, t4 < t3 -> ~ proc mch c p a t4 m) -> False).
+                                                                forall {m'}, mark mch c p a t2 m' -> recv mch c p a t3 m' -> t1 < t2 ->
+                                                                             (forall t4, t4 < t3 -> ~ recv mch c p a t4 m) -> False).
     Proof.
       intros a t.
       induction t.
@@ -608,14 +608,14 @@ Module Final (dt: DataTypes) (ch: ChannelPerAddr dt) (st: Stuff dt ch).
       intros tc tp tcLe0 tpLe0 mc msendmc mp msendmp _ _.
       assert (tcEq0: tc = 0) by omega; assert (tpEq0: tp = 0) by omega.
       rewrite tcEq0 in *; rewrite tpEq0 in *.
-      pose proof (sendmImpProcr msendmp) as [r rprocr].
-      pose proof (procImpMark rprocr) as [t' [t'Le0 rsendr]].
+      pose proof (sendmImpRecvr msendmp) as [r rrecvr].
+      pose proof (recvImpMark rrecvr) as [t' [t'Le0 rsendr]].
       assert (t'Eq0: t' = 0) by omega.
       rewrite t'Eq0 in *.
       apply (noSendmSendr st msendmc rsendr).
       constructor.
-      intros t1 t2 t3 t3Le0 m msendm r rsendr rprocr t1LeT2 neg.
-      pose proof (procImpMark rprocr) as [t5 [t5LeT3 rsendrT5]].
+      intros t1 t2 t3 t3Le0 m msendm r rsendr rrecvr t1LeT2 neg.
+      pose proof (recvImpMark rrecvr) as [t5 [t5LeT3 rsendrT5]].
       pose proof (uniqMark2 rsendr rsendrT5) as t2EqT5.
       assert (t30: t3 = 0) by omega.
       rewrite t2EqT5, t30 in *.
@@ -624,8 +624,8 @@ Module Final (dt: DataTypes) (ch: ChannelPerAddr dt) (st: Stuff dt ch).
       assert (t50: t5 = 0) by omega.
       rewrite t10, t50 in *.
       apply (noSendmSendr st msendm rsendr).
-      intros t1 t2 t3 t3Le0 m msendm m' msendm' mprocm' t1LeT2 neg.
-      pose proof (procImpMark mprocm') as [t5 [t5LeT3 msendm'T5]].
+      intros t1 t2 t3 t3Le0 m msendm m' msendm' mrecvm' t1LeT2 neg.
+      pose proof (recvImpMark mrecvm') as [t5 [t5LeT3 msendm'T5]].
       pose proof (uniqMark2 msendm' msendm'T5) as t2EqT5.
       assert (t30: t3 = 0) by omega.
       rewrite t2EqT5, t30 in *.
@@ -639,82 +639,82 @@ Module Final (dt: DataTypes) (ch: ChannelPerAddr dt) (st: Stuff dt ch).
 
       assert (cross': forall to0, to0 <= S t -> state c a to0 <= dir p c a to0).
       intros tm toLtT.
-      destruct (classical (exists ts, ts < tm /\ ((exists m, proc mch c p a ts m) \/
+      destruct (classical (exists ts, ts < tm /\ ((exists m, recv mch c p a ts m) \/
                                                   (exists m, mark mch p c a ts m)))) as [chnge|noChnge].
       pose proof (maxExists' classical chnge) as lastChnge; clear chnge.
-      destruct lastChnge as [ts [tsLtTo [procOrSend noPrevChnge]]].
+      destruct lastChnge as [ts [tsLtTo [recvOrSend noPrevChnge]]].
       assert (eq: dir p c a (S ts) = dir p c a tm) by (
                                                        assert (two: S ts = tm \/ S ts < tm) by omega;
                                                        destruct two as [eq|less]; [
                                                          intuition|
                                                          apply (@noChange (dir p c) lt p c dt); [ intuition | generalize noPrevChnge; clear; firstorder]]).
-      destruct procOrSend as [[m mprocm] | [m msendm]].
-      pose proof (procImpMark mprocm) as [t' [t'LeTs msendm]].
-      destruct (classical (exists tc, t' < tc < tm /\ exists m, proc mch p c a tc m)) as [proc|noProc].
-      destruct proc as [tc [comp [m' mprocm']]].
-      pose proof (procImpMark mprocm') as [t'' [t''LeTc msendm']].
+      destruct recvOrSend as [[m mrecvm] | [m msendm]].
+      pose proof (recvImpMark mrecvm) as [t' [t'LeTs msendm]].
+      destruct (classical (exists tc, t' < tc < tm /\ exists m, recv mch p c a tc m)) as [recv|noRecv].
+      destruct recv as [tc [comp [m' mrecvm']]].
+      pose proof (recvImpMark mrecvm') as [t'' [t''LeTc msendm']].
       assert (gOrl: t'' > ts \/ t'' <= ts) by omega.
       destruct gOrl as [t''GtTs | t''LeTs].
       assert (t''LtTc: t'' < tm) by omega.
       generalize noPrevChnge msendm' t''LtTc t''GtTs; clear; firstorder.
       assert (t'LeT: t' <= t) by omega.
       assert (t''LeT: t'' <= t) by omega.
-      assert (hyp1: forall tc', tc' < t' -> ~ proc mch p c a tc' m') by (
-                                                                         unfold not; intros tc' tc'LtT' mprocm'Tc';
-                                                                         pose proof (uniqProc2 mprocm' mprocm'Tc'); intuition).
-      assert (hyp2: forall tp', tp' < t'' -> ~ proc mch c p a tp' m) by (
-                                                                         unfold not; intros tp' tp'LtT'' mprocmTp';
-                                                                         pose proof (uniqProc2 mprocm mprocmTp'); intuition).
+      assert (hyp1: forall tc', tc' < t' -> ~ recv mch p c a tc' m') by (
+                                                                         unfold not; intros tc' tc'LtT' mrecvm'Tc';
+                                                                         pose proof (uniqRecv2 mrecvm' mrecvm'Tc'); intuition).
+      assert (hyp2: forall tp', tp' < t'' -> ~ recv mch c p a tp' m) by (
+                                                                         unfold not; intros tp' tp'LtT'' mrecvmTp';
+                                                                         pose proof (uniqRecv2 mrecvm mrecvmTp'); intuition).
       pose proof (cross t' t'' t'LeT t''LeT m msendm m' msendm' hyp1 hyp2).
       firstorder.
-      assert (noProc': ~ (exists tc, S t' <= tc < tm /\ exists m, proc mch p c a tc m /\ to m >= state c a tm)) by
+      assert (noRecv': ~ (exists tc, S t' <= tc < tm /\ exists m, recv mch p c a tc m /\ to m >= state c a tm)) by
           (
-            unfold not; intros [tc [cond [m0 [mprocm0 _]]]];
-            assert (cond': t' < tc < tm) by omega; generalize noProc cond' mprocm0; clear; firstorder).
+            unfold not; intros [tc [cond [m0 [mrecvm0 _]]]];
+            assert (cond': t' < tc < tm) by omega; generalize noRecv cond' mrecvm0; clear; firstorder).
       assert (nGt: ~ state c a tm > state c a (S t')) by (
                                                           assert (eqOrGt: tm = S t' \/ tm > S t') by omega;
                                                           destruct eqOrGt as [toEqSt' | toGtSt']; [
                                                             rewrite <- toEqSt';
                                                             omega |
                                                             pose proof (@whenChildHigh a (S t') tm toGtSt') as contra;
-                                                              generalize contra noProc'; clear; firstorder]).
+                                                              generalize contra noRecv'; clear; firstorder]).
       assert (dirEqSt: dir p c a (S ts) = state c a (S t')) by (
                                                                 pose proof (sendmChange st msendm) as one;
-                                                                pose proof (procmChange dt mprocm) as two;
+                                                                pose proof (recvmChange dt mrecvm) as two;
                                                                   congruence).
       assert (stoLesSt': state c a tm <= state c a (S t')) by omega.
       congruence.
-      pose proof (sendmImpProcr msendm) as [r rprocr].
-      pose proof (procImpMark rprocr) as [t' [t'LeTs rsendr]].
-      destruct (classical (exists tc, tc < tm /\ proc mch p c a tc m)) as [[tc [tcLtTo mprocm]] | notEx].
+      pose proof (sendmImpRecvr msendm) as [r rrecvr].
+      pose proof (recvImpMark rrecvr) as [t' [t'LeTs rsendr]].
+      destruct (classical (exists tc, tc < tm /\ recv mch p c a tc m)) as [[tc [tcLtTo mrecvm]] | notEx].
       assert (eqOrNot: tm = S tc \/ tm > S tc) by omega.
       destruct eqOrNot as [toEqStc | toGtStc].
       assert (dirEqSt: state c a tm = dir p c a tm) by (
-                                                        pose proof (sendmChange dt msendm) as one; pose proof (procmChange st mprocm) as two;
+                                                        pose proof (sendmChange dt msendm) as one; pose proof (recvmChange st mrecvm) as two;
                                                          congruence).
       omega.
-      assert (noLower: ~ exists t'', S tc <= t'' < tm /\ exists m', proc mch p c a t'' m' /\ to m' >= state c a tm)
+      assert (noLower: ~ exists t'', S tc <= t'' < tm /\ exists m', recv mch p c a t'' m' /\ to m' >= state c a tm)
         by (
-            unfold not; intros [t'' [cond [m' [mprocm' _]]]];
-            pose proof (procImpMark mprocm') as [tf [tfLeT'' msendm']];
+            unfold not; intros [t'' [cond [m' [mrecvm' _]]]];
+            pose proof (recvImpMark mrecvm') as [tf [tfLeT'' msendm']];
             assert (diff: ts = tf \/ tf < ts \/ tf > ts) by omega;
             destruct diff as [tsEqTf | [tfLtTs | tfGtTs]]; [
               rewrite <- tsEqTf in *;
               pose proof (uniqMark1 msendm msendm') as mEqM';
               rewrite <- mEqM' in *;
-              pose proof (uniqProc2 mprocm mprocm') as tcEqT'';
+              pose proof (uniqRecv2 mrecvm mrecvm') as tcEqT'';
               omega |
               assert (t'LeTc: t' <= tc) by (
-                                            pose proof (procImpMark mprocm) as [tsome [tsomeLe'' msendmTsome]];
+                                            pose proof (recvImpMark mrecvm) as [tsome [tsomeLe'' msendmTsome]];
                                             pose proof (uniqMark2 msendm msendmTsome) as tcEqTsome;
                                             rewrite <- tcEqTsome in *; omega);
                 pose proof @cReqPRespCross;
-                assert (cross1: forall tc', tc' < t' -> ~ proc mch p c a tc' m') by (
-                                                                                     unfold not; intros tc' tc'LtT' mprocm'Tc';
-                                                                                     pose proof (uniqProc2 mprocm' mprocm'Tc') as t'EqTc'; omega);
-                assert (cross2: forall tp', tp' <= tf -> ~ proc rch c p a tp' r) by (
-                                                                                     unfold not; intros tp' tp'LeTf rprocrTp';
-                                                                                     pose proof (uniqProc2 rprocr rprocrTp') as tfEqTp'; omega);
+                assert (cross1: forall tc', tc' < t' -> ~ recv mch p c a tc' m') by (
+                                                                                     unfold not; intros tc' tc'LtT' mrecvm'Tc';
+                                                                                     pose proof (uniqRecv2 mrecvm' mrecvm'Tc') as t'EqTc'; omega);
+                assert (cross2: forall tp', tp' <= tf -> ~ recv rch c p a tp' r) by (
+                                                                                     unfold not; intros tp' tp'LeTf rrecvrTp';
+                                                                                     pose proof (uniqRecv2 rrecvr rrecvrTp') as tfEqTp'; omega);
                 assert (t''LeT: t'' <= t) by omega;
                 assert (tfLeT: tf <= t) by omega;
                 apply (cReqPRespCross rsendr msendm' cross1 cross2)|
@@ -724,53 +724,53 @@ Module Final (dt: DataTypes) (ch: ChannelPerAddr dt) (st: Stuff dt ch).
       assert (not: ~ state c a tm > state c a (S tc)) by (generalize noLower contra; clear; firstorder).
       assert (not2: state c a tm <= state c a (S tc)) by omega; clear not.
       assert (dirEqSt: dir p c a (S ts) = state c a (S tc)) by (
-                                                                pose proof (sendmChange dt msendm) as one; pose proof (procmChange st mprocm) as two;
+                                                                pose proof (sendmChange dt msendm) as one; pose proof (recvmChange st mrecvm) as two;
                                                                 congruence).
       omega.
       assert (tsLeT: ts <= t) by omega.
       assert (less: state c a ts <= dir p c a ts) by firstorder.
       assert (tmGtTs: tm > t') by omega.
-      assert (noProc: ~ exists t'', t' <= t'' < tm /\ exists m, proc mch p c a t'' m /\ to m >= state c a tm) by (
-                                                                                                                  unfold not; intros [t'' [cond [m' [mprocm' _]]]];
-                                                                                                                  pose proof (procImpMark mprocm') as [t1 [t1LeT'' msendm']];
+      assert (noRecv: ~ exists t'', t' <= t'' < tm /\ exists m, recv mch p c a t'' m /\ to m >= state c a tm) by (
+                                                                                                                  unfold not; intros [t'' [cond [m' [mrecvm' _]]]];
+                                                                                                                  pose proof (recvImpMark mrecvm') as [t1 [t1LeT'' msendm']];
                                                                                                                   assert (t1NeTs: t1 = ts -> False) by (
                                                                                                                                                         intros t1EqTs; rewrite t1EqTs in *;
                                                                                                                                                                        pose proof (uniqMark1 msendm msendm') as mEqm';
                                                                                                                                                         rewrite <- mEqm' in *; 
-                                                                                                                                                          generalize notEx cond mprocm'; clear; firstorder);
+                                                                                                                                                          generalize notEx cond mrecvm'; clear; firstorder);
                                                                                                                   assert (eqOrNot: t1 = ts \/ t1 > ts \/ t1 < ts) by omega;
                                                                                                                   destruct eqOrNot as [t1EqTs | [t1GtTs | t1LtTs]];
                                                                                                                   [firstorder |
                                                                                                                    assert (cond2: ts < t1 < tm) by omega;
                                                                                                                      generalize noPrevChnge cond2 msendm'; clear; firstorder |
-                                                                                                                   assert (one: forall tc', tc' < t' -> ~ proc mch p c a tc' m') by (
-                                                                                                                                                                                     unfold not; intros tc' tc'LtT' mprocm'Tc';
-                                                                                                                                                                                     pose proof (uniqProc2 mprocm' mprocm'Tc') as t''EqTc'; omega);
-                                                                                                                     assert (two: forall tp', tp' <= t1 -> ~ proc rch c p a tp' r) by (
-                                                                                                                                                                                       unfold not; intros tp' tp'LeT1 rprocrTp';
-                                                                                                                                                                                       pose proof (uniqProc2 rprocr rprocrTp') as tsEqTp'; omega);
+                                                                                                                   assert (one: forall tc', tc' < t' -> ~ recv mch p c a tc' m') by (
+                                                                                                                                                                                     unfold not; intros tc' tc'LtT' mrecvm'Tc';
+                                                                                                                                                                                     pose proof (uniqRecv2 mrecvm' mrecvm'Tc') as t''EqTc'; omega);
+                                                                                                                     assert (two: forall tp', tp' <= t1 -> ~ recv rch c p a tp' r) by (
+                                                                                                                                                                                       unfold not; intros tp' tp'LeT1 rrecvrTp';
+                                                                                                                                                                                       pose proof (uniqRecv2 rrecvr rrecvrTp') as tsEqTp'; omega);
                                                                                                                      apply (cReqPRespCross rsendr msendm' one two)]).
       assert (contra1: ~ state c a tm > state c a t') by (
                                                           unfold not; intros contra;
-                                                          generalize (whenChildHigh tmGtTs contra) noProc; clear; firstorder).
+                                                          generalize (whenChildHigh tmGtTs contra) noRecv; clear; firstorder).
       assert (cont: state c a tm <= state c a t') by omega.
       pose proof (sendrImpSt st rsendr) as toRGtDir.
-      pose proof (sendmImpProcrGe msendm rprocr) as toMGeToR.
+      pose proof (sendmImpRecvrGe msendm rrecvr) as toMGeToR.
       pose proof (sendmChange dt msendm) as toMEq.
       omega.
       assert (eqOrNot: 0 = tm \/ 0 < tm) by omega.
       destruct eqOrNot as [tmEq0 | tmGt0].
       rewrite <- tmEq0 in *; pose proof @init as init; rewrite init in *; omega.
       assert (premise: forall tn, 0 <= tn < tm -> (forall m, ~ mark mch p c a tn m) /\
-                                                  (forall m, ~ proc mch c p a tn m)) by (
+                                                  (forall m, ~ recv mch c p a tn m)) by (
                                                                                          intros tn [_ tnLtTm];
                                                                                          constructor;
                                                                                          unfold not; intros m msendm;
                                                                                          generalize noChnge tnLtTm msendm; clear; firstorder).
       pose proof (noChange dt tmGt0 premise) as dir0DirTm.
-      assert (not: ~ exists t'', 0 <= t'' < tm /\ exists m, proc mch p c a t'' m /\ to m >= state c a tm) by (
-                                                                                                              unfold not; intros [t'' [[_ t''LtTm] [m [mprocm _]]]];
-                                                                                                              pose proof (procImpMark mprocm) as [t' [t'LeT'' msendm]];
+      assert (not: ~ exists t'', 0 <= t'' < tm /\ exists m, recv mch p c a t'' m /\ to m >= state c a tm) by (
+                                                                                                              unfold not; intros [t'' [[_ t''LtTm] [m [mrecvm _]]]];
+                                                                                                              pose proof (recvImpMark mrecvm) as [t' [t'LeT'' msendm]];
                                                                                                               assert (t'LtTm: t' < tm) by omega;
                                                                                                               generalize noChnge t'LtTm msendm; clear; firstorder).
       assert (done: ~ state c a tm > state c a 0) by (generalize (@whenChildHigh a 0 tm tmGt0) not;
@@ -781,34 +781,34 @@ Module Final (dt: DataTypes) (ch: ChannelPerAddr dt) (st: Stuff dt ch).
       apply cross'.
 
       assert (cReqResp': forall {t1 t2 t3}, t3 <= S t -> forall {m}, mark mch c p a t1 m -> forall {r},
-                                                                                              mark rch c p a t2 r -> proc rch c p a t3 r -> t1 <= t2 -> (forall t4, t4 < t3 -> ~ proc mch c p a t4 m) ->
+                                                                                              mark rch c p a t2 r -> recv rch c p a t3 r -> t1 <= t2 -> (forall t4, t4 < t3 -> ~ recv mch c p a t4 m) ->
                                                                                               False).
-      intros t1 t2 t3 t3LeSt m msendm r rsendr rprocr t1LeT2 neg.
+      intros t1 t2 t3 t3LeSt m msendm r rsendr rrecvr t1LeT2 neg.
       unfold Time in *.
       assert (eqOrNot: t1 = t2 \/ t1 < t2) by omega.
       destruct eqOrNot as [t1EqT2 | t1LtT2].
       rewrite t1EqT2 in *.
       pose proof (noSendmSendr st msendm rsendr); intuition.
       clear t1LeT2.
-      pose proof (procImpMark rprocr) as [t' [t'LeT3 rsend'r]].
+      pose proof (recvImpMark rrecvr) as [t' [t'LeT3 rsend'r]].
       pose proof (uniqMark2 rsendr rsend'r) as t2EqT'.
       rewrite <- t2EqT' in *.
       clear rsend'r t2EqT'.
       assert (t1LeT: t1 <= t) by omega.
       pose proof (cons t1 t1LeT) as st1Ledt1.
 
-      assert (notty1: ~ exists t'', t1 <= t'' < t2 /\ exists m, proc mch p c a t'' m /\ to m >= state c a t2) by (
-                                                                                                                  unfold not; intros [t'' [cond [m0 [mprocm0 _]]]];
-                                                                                                                  pose proof (procImpMark mprocm0) as [t5 [t5LeT'' msendm0]];
-                                                                                                                  assert (one: forall tc', tc' < t1 -> ~ proc mch p c a tc' m0) by (
-                                                                                                                                                                                    unfold not; intros tc' tc'LtT1 mprocM0Tc';
-                                                                                                                                                                                    pose proof (uniqProc2 mprocm0 mprocM0Tc') as t''EqTc';
+      assert (notty1: ~ exists t'', t1 <= t'' < t2 /\ exists m, recv mch p c a t'' m /\ to m >= state c a t2) by (
+                                                                                                                  unfold not; intros [t'' [cond [m0 [mrecvm0 _]]]];
+                                                                                                                  pose proof (recvImpMark mrecvm0) as [t5 [t5LeT'' msendm0]];
+                                                                                                                  assert (one: forall tc', tc' < t1 -> ~ recv mch p c a tc' m0) by (
+                                                                                                                                                                                    unfold not; intros tc' tc'LtT1 mrecvM0Tc';
+                                                                                                                                                                                    pose proof (uniqRecv2 mrecvm0 mrecvM0Tc') as t''EqTc';
                                                                                                                                                                                     rewrite <- t''EqTc' in *; omega);
-                                                                                                                  assert (two: forall tp', tp' < t5 -> ~ proc mch c p a tp' m) by (
+                                                                                                                  assert (two: forall tp', tp' < t5 -> ~ recv mch c p a tp' m) by (
                                                                                                                                                                                    unfold not; intros tp' tp'LtT5; assert (t5LtT3: tp' < t3) by omega; firstorder);
                                                                                                                   assert (t5Let: t5 <= t) by omega;
                                                                                                                   apply (cross t1 t5 t1LeT t5Let m msendm m0 msendm0 one two)).
-      assert (notty: ~ exists t'', S t1 <= t'' < t2 /\ exists m, proc mch p c a t'' m /\ to m >= state c a t2) by (
+      assert (notty: ~ exists t'', S t1 <= t'' < t2 /\ exists m, recv mch p c a t'' m /\ to m >= state c a t2) by (
                                                                                                                    clear cRespResp;
                                                                                                                    unfold not; intros [t'' [cond ex]];
                                                                                                                    assert (cond2: t1 <= t'' < t2) by omega;
@@ -822,60 +822,60 @@ Module Final (dt: DataTypes) (ch: ChannelPerAddr dt) (st: Stuff dt ch).
                                                                     omega|
                                                                     unfold not; intros st; pose proof (whenChildHigh St1LtT2 st) as some; firstorder]).
       assert (stt2LestT1: state c a t2 <= state c a (S t1)) by omega.
-      pose proof (procrCond rprocr) as fromRLe.
+      pose proof (recvrCond rrecvr) as fromRLe.
       pose proof (sendrFrom st rsendr) as fromREq.
       pose proof (sendmImpSt msendm) as stGt.
       pose proof (sendmChange st msendm) as stEq.
       rewrite fromREq, <- stEq in *.
       assert (drGt: dir p c a t1 > dir p c a t3) by omega.
       assert (drNe: dir p c a t1 <> dir p c a t3) by omega.
-      assert (sendProc: ~ forall tn, t1 <= tn < t3 -> (forall m, ~ mark mch p c a tn m) /\
-                                                      (forall m, ~ proc mch c p a tn m)) by (
+      assert (sendRecv: ~ forall tn, t1 <= tn < t3 -> (forall m, ~ mark mch p c a tn m) /\
+                                                      (forall m, ~ recv mch c p a tn m)) by (
                                                                                              unfold not; intros exp; assert (t1LtT3: t1 < t3) by omega; pose proof (noChange dt t1LtT3 exp); firstorder).
       assert (noSend: forall tn, t1 <= tn < t3 -> forall m, ~ mark mch p c a tn m) by (
                                                                                        clear cRespResp;
                                                                                        unfold not; intros tn cond m0 msendm0;
                                                                                        assert (tnLeT: tn <= t) by omega;
-                                                                                       assert (one: forall tc', tc' < t1 -> ~ proc mch p c a tc' m0) by (
-                                                                                                                                                         unfold not; intros tc' tc'LtT1 mprocm0;
-                                                                                                                                                         pose proof (procImpMark mprocm0) as [tm [tmLeTc' msend'm0]];
+                                                                                       assert (one: forall tc', tc' < t1 -> ~ recv mch p c a tc' m0) by (
+                                                                                                                                                         unfold not; intros tc' tc'LtT1 mrecvm0;
+                                                                                                                                                         pose proof (recvImpMark mrecvm0) as [tm [tmLeTc' msend'm0]];
                                                                                                                                                          pose proof (uniqMark2 msendm0 msend'm0) as tmEqTc';
                                                                                                                                                          rewrite <- tmEqTc' in *; omega);
-                                                                                       assert (two: forall tp', tp' < tn -> ~ proc mch c p a tp' m) by (
+                                                                                       assert (two: forall tp', tp' < tn -> ~ recv mch c p a tp' m) by (
                                                                                                                                                         unfold not; intros tp' tp'LtTn; assert (tp'LtT3: tp' < t3) by omega; firstorder);
                                                                                        apply (cross t1 tn t1LeT tnLeT m msendm m0 msendm0 one two)).
 
-      destruct (classical (exists tn, tn < t3 /\ t1 <= tn /\ exists m0, proc mch c p a tn m0)) as [ext|noEx].
-      pose proof (maxExists' classical ext) as [tn [cond [[tnLtT3 [m0 mprocm0]] notAfter]]].
+      destruct (classical (exists tn, tn < t3 /\ t1 <= tn /\ exists m0, recv mch c p a tn m0)) as [ext|noEx].
+      pose proof (maxExists' classical ext) as [tn [cond [[tnLtT3 [m0 mrecvm0]] notAfter]]].
       
-      pose proof (procImpMark mprocm0) as [tr [trLeTn msendm0]].
+      pose proof (recvImpMark mrecvm0) as [tr [trLeTn msendm0]].
       assert (opts: tr = t1 \/ tr > t1 \/ tr < t1) by omega.
       destruct opts as [trEqT1 | [trGtT1 | trLtT1]].
       rewrite trEqT1 in *.
       pose proof (uniqMark1 msendm msendm0) as mEqm0.
       rewrite <- mEqm0 in *.
-      generalize neg cond mprocm0; clear; firstorder.
+      generalize neg cond mrecvm0; clear; firstorder.
       assert (tnLeT: tn <= t) by omega.
-      assert (cond2: forall t4, t4 < tn -> ~ proc mch c p a t4 m) by (
+      assert (cond2: forall t4, t4 < tn -> ~ recv mch c p a t4 m) by (
                                                                       intros t4 t4LtTn; assert (t4LtT3: t4 < t3) by omega;
                                                                       generalize neg t4LtT3; clear; firstorder).
-      apply (cRespResp t1 tr tn tnLeT m msendm m0 msendm0 mprocm0 trGtT1 cond2).
-      assert (notty2': ~ exists t'', tr <= t'' < t1 /\ exists m, proc mch p c a t'' m /\ to m >= state c a t1) by (
-                                                                                                                   unfold not; intros [t'' [cond2 [m1 [mprocm1 _]]]];
-                                                                                                                   pose proof (procImpMark mprocm1) as [t5 [t5LeT'' msendm1]];
+      apply (cRespResp t1 tr tn tnLeT m msendm m0 msendm0 mrecvm0 trGtT1 cond2).
+      assert (notty2': ~ exists t'', tr <= t'' < t1 /\ exists m, recv mch p c a t'' m /\ to m >= state c a t1) by (
+                                                                                                                   unfold not; intros [t'' [cond2 [m1 [mrecvm1 _]]]];
+                                                                                                                   pose proof (recvImpMark mrecvm1) as [t5 [t5LeT'' msendm1]];
                                                                                                                    assert (trLeT: tr <= t) by omega;
                                                                                                                    assert (t5LeT: t5 <= t) by omega;
-                                                                                                                   assert (one: forall tc', tc' < tr -> ~ proc mch p c a tc' m1) by (
-                                                                                                                                                                                     unfold not; intros tc' tc'LtTr mproc'm1;
-                                                                                                                                                                                     pose proof (uniqProc2 mprocm1 mproc'm1) as t''EqTc';
+                                                                                                                   assert (one: forall tc', tc' < tr -> ~ recv mch p c a tc' m1) by (
+                                                                                                                                                                                     unfold not; intros tc' tc'LtTr mrecv'm1;
+                                                                                                                                                                                     pose proof (uniqRecv2 mrecvm1 mrecv'm1) as t''EqTc';
                                                                                                                                                                                      rewrite <- t''EqTc' in *;
                                                                                                                                                                                        omega);
-                                                                                                                   assert (two: forall tp', tp' < t5 -> ~ proc mch c p a tp' m0) by (
-                                                                                                                                                                                     unfold not; intros tp' tp'LtT5 mproc'm0;
-                                                                                                                                                                                     pose proof (uniqProc2 mprocm0 mproc'm0) as tnEqTp';
+                                                                                                                   assert (two: forall tp', tp' < t5 -> ~ recv mch c p a tp' m0) by (
+                                                                                                                                                                                     unfold not; intros tp' tp'LtT5 mrecv'm0;
+                                                                                                                                                                                     pose proof (uniqRecv2 mrecvm0 mrecv'm0) as tnEqTp';
                                                                                                                                                                                      rewrite <- tnEqTp' in *; omega);
                                                                                                                    apply (cross tr t5 trLeT t5LeT m0 msendm0 m1 msendm1 one two)).
-      assert (notty2: ~ exists t'', S tr <= t'' < t1 /\ exists m, proc mch p c a t'' m /\ to m >= state c a t1) by (
+      assert (notty2: ~ exists t'', S tr <= t'' < t1 /\ exists m, recv mch p c a t'' m /\ to m >= state c a t1) by (
                                                                                                                     unfold not; intros [t'' [cond1 rest]]; assert (cond2: tr <= t'' < t1) by omega;
                                                                                                                     generalize notty2' cond2 rest; clear; firstorder).
       assert (strLeT1: S tr <= t1) by omega.
@@ -883,66 +883,66 @@ Module Final (dt: DataTypes) (ch: ChannelPerAddr dt) (st: Stuff dt ch).
       pose proof (whenChildHighConv t1LtT2 notty) as sST1LeT2.
       assert (trLtT3: tr < t3) by omega.
       assert (noC: forall tn0, S tn <= tn0 < t3 -> (forall m, ~ mark mch p c a tn0 m) /\
-                                                   (forall m, ~ proc mch c p a tn0 m)) by (
+                                                   (forall m, ~ recv mch c p a tn0 m)) by (
                                                                                            intros tn0 cond2;
                                                                                            constructor; [assert (cond3: t1 <= tn0 < t3) by omega; generalize noSend cond3; clear; firstorder|
                                                                                                          assert (cond4: tn < tn0 < t3) by omega; 
                                                                                                            assert (t1LeTn0: t1 <= tn0) by omega; generalize cond4 t1LeTn0 notAfter; clear; firstorder]).
       assert (sTnLtT3: S tn <= t3) by omega.
       pose proof (noChange2 dt sTnLtT3 noC) as dirEq.
-      generalize st1LeTr sST1LeT2 sTnLtT3 dirEq rsendr rprocr msendm msendm0 mprocm0; clear; intros.
+      generalize st1LeTr sST1LeT2 sTnLtT3 dirEq rsendr rrecvr msendm msendm0 mrecvm0; clear; intros.
       pose proof (sendmChange st msendm) as sEqTom.
       pose proof (sendmImpSt msendm) as sGtTom.
-      pose proof (procmChange dt mprocm0) as dSEqTom0.
+      pose proof (recvmChange dt mrecvm0) as dSEqTom0.
       pose proof (sendmChange st msendm0) as sSEqTom0.
-      pose proof (procrCond rprocr) as dLeFromr.
+      pose proof (recvrCond rrecvr) as dLeFromr.
       pose proof (sendrFrom st rsendr) as sEqFromr.
       omega.
-      generalize sendProc noSend noEx; clear; firstorder.
+      generalize sendRecv noSend noEx; clear; firstorder.
 
       constructor.
 
-      intros tc tp tcLeSt tpLeSt mc msendmc mp msendmp noprocmp noprocmc.
-      pose proof (sendmImpProcr msendmp) as [r rprocr].
-      pose proof (procImpMark rprocr) as [t1 [t1LeTp rsendr]].
+      intros tc tp tcLeSt tpLeSt mc msendmc mp msendmp norecvmp norecvmc.
+      pose proof (sendmImpRecvr msendmp) as [r rrecvr].
+      pose proof (recvImpMark rrecvr) as [t1 [t1LeTp rsendr]].
       assert (opts: t1 = tc \/ tc < t1 \/ t1 < tc) by omega.
       destruct opts as [t1EqTc | [tcLtT1 | t1LtTc]].
       rewrite t1EqTc in *.
       apply (noSendmSendr st msendmc rsendr).
       assert (tcLeT1: tc <= t1) by omega.
-      apply (cReqResp' tc t1 tp tpLeSt mc msendmc r rsendr rprocr tcLeT1 noprocmc).
-      destruct (classical (exists tm, t1 <= tm < tc /\ exists m, proc mch p c a tm m)) as [ext|noExt].
-      destruct ext as [tm [[t1LeTm tmLtTc] [m procm]]].
-      pose proof (procImpMark procm) as [tn [tnLeTm sendm]].
+      apply (cReqResp' tc t1 tp tpLeSt mc msendmc r rsendr rrecvr tcLeT1 norecvmc).
+      destruct (classical (exists tm, t1 <= tm < tc /\ exists m, recv mch p c a tm m)) as [ext|noExt].
+      destruct ext as [tm [[t1LeTm tmLtTc] [m recvm]]].
+      pose proof (recvImpMark recvm) as [tn [tnLeTm sendm]].
       assert (opts: tn = tp \/ tn < tp \/ tn > tp) by omega.
       destruct opts as [tnEqTp | [tnLtTp | tnGtTp]].
       rewrite tnEqTp in *.
       pose proof (uniqMark1 sendm msendmp) as mEqMp.
       rewrite mEqMp in *.
       firstorder.
-      assert (one: forall tc', tc' < t1 -> ~ proc mch p c a tc' m) by (
-                                                                       unfold not; intros tc' tc'LtT1 proc'm;
-                                                                       pose proof (uniqProc2 procm proc'm) as tmEqTc';
+      assert (one: forall tc', tc' < t1 -> ~ recv mch p c a tc' m) by (
+                                                                       unfold not; intros tc' tc'LtT1 recv'm;
+                                                                       pose proof (uniqRecv2 recvm recv'm) as tmEqTc';
                                                                        omega).
-      assert (two: forall tp', tp' <= tn -> ~ proc rch c p a tp' r) by (
-                                                                        unfold not; intros tp' tp'LeTn proc'r;
-                                                                        pose proof (uniqProc2 rprocr proc'r) as tpEqTp';
+      assert (two: forall tp', tp' <= tn -> ~ recv rch c p a tp' r) by (
+                                                                        unfold not; intros tp' tp'LeTn recv'r;
+                                                                        pose proof (uniqRecv2 rrecvr recv'r) as tpEqTp';
                                                                         omega).
       apply (cReqPRespCross rsendr sendm one two).
-      pose proof (sendmImpProcr sendm) as [r1 procr1].
-      pose proof (procImpMark procr1) as [tq [tqLeTn sendr1]].
-      assert (one: forall tc', tc' < tq -> ~ proc mch p c a tc' mp) by (
+      pose proof (sendmImpRecvr sendm) as [r1 recvr1].
+      pose proof (recvImpMark recvr1) as [tq [tqLeTn sendr1]].
+      assert (one: forall tc', tc' < tq -> ~ recv mch p c a tc' mp) by (
                                                                         unfold not; intros tc' tc'LtTq; assert (tc'LtTc: tc' < tc) by omega;
-                                                                        apply (noprocmp tc' tc'LtTc)).
-      assert (two: forall tp', tp' <= tp -> ~ proc rch c p a tp' r1) by (
-                                                                         unfold not; intros tp' tp'LeTp proc'r1;
-                                                                         pose proof (uniqProc2 procr1 proc'r1) as tpEqTp';
+                                                                        apply (norecvmp tc' tc'LtTc)).
+      assert (two: forall tp', tp' <= tp -> ~ recv rch c p a tp' r1) by (
+                                                                         unfold not; intros tp' tp'LeTp recv'r1;
+                                                                         pose proof (uniqRecv2 recvr1 recv'r1) as tpEqTp';
                                                                          omega).
       apply (cReqPRespCross sendr1 msendmp one two).
-      assert (opt: ~ exists tm, t1 <= tm < tc /\ exists m, proc mch p c a tm m) by (
+      assert (opt: ~ exists tm, t1 <= tm < tc /\ exists m, recv mch p c a tm m) by (
                                                                                     generalize noExt; clear; firstorder).
       assert (opt': forall t', t1 < t' <= tc -> ~ exists tm, t1 <= tm < t' /\ exists m,
-                                                                                proc mch p c a tm m /\ to m >= state c a t') by (
+                                                                                recv mch p c a tm m /\ to m >= state c a t') by (
                                                                                                                                  unfold not; intros t' t'LtTc [tm [cond rest]]; assert (cond2: t1 <= tm < tc) by omega;
                                                                                                                                  generalize opt t'LtTc cond2 rest; clear; firstorder).
       assert (notSth: forall t', t1 < t' <= tc -> ~ state c a t' > state c a t1) by (
@@ -956,17 +956,17 @@ Module Final (dt: DataTypes) (ch: ChannelPerAddr dt) (st: Stuff dt ch).
       assert (stcLet2: forall t', t1 < t' <= tc -> state c a t' < to r) by (
                                                                             intros t' cond; specialize (stcLet1 t' cond); omega).
       clear stcLet1 gtRel.
-      pose proof (voluntary rsendr t1LtTc msendmc stcLet2) as [r1 [procr1 sTcGtToR1]].
-      pose proof (procImpMark procr1) as [t2 [t2LeT1 sendr1]].
+      pose proof (voluntary rsendr t1LtTc msendmc stcLet2) as [r1 [recvr1 sTcGtToR1]].
+      pose proof (recvImpMark recvr1) as [t2 [t2LeT1 sendr1]].
       assert (t2LeTp: t2 = tp \/ t2 > tp \/ t2 < tp) by omega.
       destruct t2LeTp as [t2EqTp | [t2GtTp | t2LtTp]].
       rewrite t2EqTp in *.
       apply (noSendmSendr dt msendmp sendr1).
       assert (tpLeT2: tp <= t2) by omega.
-      pose proof (pRespReq noTwoPResp noTwoPReqNon msendmp sendr1 procr1 tpLeT2) as [t4 [t4LtTp procmp]].
-      generalize noprocmp procmp t4LtTp; clear; firstorder.
-      pose proof (sendrImpNoSendm t2LtTp sendr1 msendmp) as [t' [[t2LtT' t'LtTp] [m [procm toMGeToR1]]]].
-      pose proof (procImpMark procm) as [t'' [t''LeT' sendm]].
+      pose proof (pRespReq noTwoPResp noTwoPReqNon msendmp sendr1 recvr1 tpLeT2) as [t4 [t4LtTp recvmp]].
+      generalize norecvmp recvmp t4LtTp; clear; firstorder.
+      pose proof (sendrImpNoSendm t2LtTp sendr1 msendmp) as [t' [[t2LtT' t'LtTp] [m [recvm toMGeToR1]]]].
+      pose proof (recvImpMark recvm) as [t'' [t''LeT' sendm]].
       pose proof (sendmChange st sendm) as stEqToM.
       assert (stTcGtStST'': state c a tc > state c a (S t'')) by omega.
       assert (opts: t'' = tc \/ t'' > tc \/ t'' < tc) by omega.
@@ -974,66 +974,66 @@ Module Final (dt: DataTypes) (ch: ChannelPerAddr dt) (st: Stuff dt ch).
       rewrite t''EqTc in *.
       pose proof (uniqMark1 msendmc sendm) as mEqMc.
       rewrite mEqMc in *.
-      generalize t'LtTp procm noprocmc; clear; firstorder.
+      generalize t'LtTp recvm norecvmc; clear; firstorder.
       assert (t'Let: t' <= t) by omega.
-      assert (noproc: forall t4, t4 < t' -> ~ proc mch c p a t4 mc) by (
+      assert (norecv: forall t4, t4 < t' -> ~ recv mch c p a t4 mc) by (
                                                                         unfold not; intros t4 t4LtT'; assert (t4LtTp: t4 < tp) by omega;
-                                                                        generalize noprocmc t4LtTp; clear; firstorder).
-      apply (cRespResp tc t'' t' t'Let mc msendmc m sendm procm t''GtTc); intuition.
+                                                                        generalize norecvmc t4LtTp; clear; firstorder).
+      apply (cRespResp tc t'' t' t'Let mc msendmc m sendm recvm t''GtTc); intuition.
       assert (opts: S t'' = tc \/ S t'' < tc) by omega.
       destruct opts as [St''EqTc | St''LtTc].
       rewrite St''EqTc in *.
       omega.
-      pose proof (whenChildHigh St''LtTc stTcGtStST'') as [ts [cond [s [procs _]]]].
-      pose proof (procImpMark procs) as [tsr [tsrLeTs sends]].
+      pose proof (whenChildHigh St''LtTc stTcGtStST'') as [ts [cond [s [recvs _]]]].
+      pose proof (recvImpMark recvs) as [tsr [tsrLeTs sends]].
       assert (opts: tsr = t' \/ tsr > t' \/ tsr < t') by omega.
       destruct opts as [tsrEqT' | [tsrGtT' | tsrLtT']].
       rewrite tsrEqT' in *.
-      apply (noSendmProcm dt sends procm).
+      apply (noSendmRecvm dt sends recvm).
       assert (t2LeTsr: t2 <= tsr) by omega.
-      pose proof (pReqResp noTwoPResp noTwoPReqNon sendr1 sends procs t2LeTsr) as [tf [tfLtTs proc'r1]].
+      pose proof (pReqResp noTwoPResp noTwoPReqNon sendr1 sends recvs t2LeTsr) as [tf [tfLtTs recv'r1]].
       assert (tfLtTc: tf < tc) by omega.
-      pose proof (uniqProc2 procr1 proc'r1) as tcEqTf.
+      pose proof (uniqRecv2 recvr1 recv'r1) as tcEqTf.
       omega.
       assert (t''LeT: t'' <= t) by omega.
       assert (tsrLeT: tsr <= t) by omega.
-      assert (one: forall tc', tc' < t'' -> ~ proc mch p c a tc' s) by (
-                                                                        unfold not; intros tc' tc'LtT'' proc's; pose proof (uniqProc2 procs proc's) as tc'EqT';
+      assert (one: forall tc', tc' < t'' -> ~ recv mch p c a tc' s) by (
+                                                                        unfold not; intros tc' tc'LtT'' recv's; pose proof (uniqRecv2 recvs recv's) as tc'EqT';
                                                                         rewrite tc'EqT' in *; omega).
-      assert (two: forall tp', tp' < tsr -> ~ proc mch c p a tp' m) by (
-                                                                        unfold not; intros tp' tp'LtTsr proc'm; pose proof (uniqProc2 procm proc'm) as tp'EqTsr;
+      assert (two: forall tp', tp' < tsr -> ~ recv mch c p a tp' m) by (
+                                                                        unfold not; intros tp' tp'LtTsr recv'm; pose proof (uniqRecv2 recvm recv'm) as tp'EqTsr;
                                                                         omega).
       apply (cross t'' tsr t''LeT tsrLeT  m sendm s sends one two).
 
       constructor.
       intuition.
 
-      intros t1 t2 t3 t3LeSt m msendm r rsendr rprocr t1LeT2 neg.
+      intros t1 t2 t3 t3LeSt m msendm r rsendr rrecvr t1LeT2 neg.
       unfold Time in *.
       assert (eqOrNot: t1 = t2 \/ t1 < t2) by omega.
       destruct eqOrNot as [t1EqT2 | t1LtT2].
       rewrite t1EqT2 in *.
       pose proof (uniqMark1 msendm rsendr) as mEqR; omega.
       clear t1LeT2.
-      pose proof (procImpMark rprocr) as [t' [t'LeT3 rsend'r]].
+      pose proof (recvImpMark rrecvr) as [t' [t'LeT3 rsend'r]].
       pose proof (uniqMark2 rsendr rsend'r) as t2EqT'.
       rewrite <- t2EqT' in *.
       clear rsend'r t2EqT'.
       assert (t1LeT: t1 <= t) by omega.
       pose proof (cons t1 t1LeT) as st1Ledt1.
 
-      assert (notty1: ~ exists t'', t1 <= t'' < t2 /\ exists m, proc mch p c a t'' m /\ to m >= state c a t2) by (
-                                                                                                                  unfold not; intros [t'' [cond [m0 [mprocm0 _]]]];
-                                                                                                                  pose proof (procImpMark mprocm0) as [t5 [t5LeT'' msendm0]];
-                                                                                                                  assert (one: forall tc', tc' < t1 -> ~ proc mch p c a tc' m0) by (
-                                                                                                                                                                                    unfold not; intros tc' tc'LtT1 mprocM0Tc';
-                                                                                                                                                                                    pose proof (uniqProc2 mprocm0 mprocM0Tc') as t''EqTc';
+      assert (notty1: ~ exists t'', t1 <= t'' < t2 /\ exists m, recv mch p c a t'' m /\ to m >= state c a t2) by (
+                                                                                                                  unfold not; intros [t'' [cond [m0 [mrecvm0 _]]]];
+                                                                                                                  pose proof (recvImpMark mrecvm0) as [t5 [t5LeT'' msendm0]];
+                                                                                                                  assert (one: forall tc', tc' < t1 -> ~ recv mch p c a tc' m0) by (
+                                                                                                                                                                                    unfold not; intros tc' tc'LtT1 mrecvM0Tc';
+                                                                                                                                                                                    pose proof (uniqRecv2 mrecvm0 mrecvM0Tc') as t''EqTc';
                                                                                                                                                                                     rewrite <- t''EqTc' in *; omega);
-                                                                                                                  assert (two: forall tp', tp' < t5 -> ~ proc mch c p a tp' m) by (
+                                                                                                                  assert (two: forall tp', tp' < t5 -> ~ recv mch c p a tp' m) by (
                                                                                                                                                                                    unfold not; intros tp' tp'LtT5; assert (t5LtT3: tp' < t3) by omega; firstorder);
                                                                                                                   assert (t5Let: t5 <= t) by omega;
                                                                                                                   apply (cross t1 t5 t1LeT t5Let m msendm m0 msendm0 one two)).
-      assert (notty: ~ exists t'', S t1 <= t'' < t2 /\ exists m, proc mch p c a t'' m /\ to m >= state c a t2) by (
+      assert (notty: ~ exists t'', S t1 <= t'' < t2 /\ exists m, recv mch p c a t'' m /\ to m >= state c a t2) by (
                                                                                                                    clear cRespResp;
                                                                                                                    unfold not; intros [t'' [cond ex]];
                                                                                                                    assert (cond2: t1 <= t'' < t2) by omega;
@@ -1047,60 +1047,60 @@ Module Final (dt: DataTypes) (ch: ChannelPerAddr dt) (st: Stuff dt ch).
                                                                     omega|
                                                                     unfold not; intros st; pose proof (whenChildHigh St1LtT2 st) as some; firstorder]).
       assert (stt2LestT1: state c a t2 <= state c a (S t1)) by omega.
-      pose proof (procmCond rprocr) as fromRLe.
+      pose proof (recvmCond rrecvr) as fromRLe.
       pose proof (sendmFrom st rsendr) as fromREq.
       pose proof (sendmImpSt msendm) as stGt.
       pose proof (sendmChange st msendm) as stEq.
       rewrite fromREq, <- stEq in *.
       assert (drGt: dir p c a t1 > dir p c a t3) by omega.
       assert (drNe: dir p c a t1 <> dir p c a t3) by omega.
-      assert (sendProc: ~ forall tn, t1 <= tn < t3 -> (forall m, ~ mark mch p c a tn m) /\
-                                                      (forall m, ~ proc mch c p a tn m)) by (
+      assert (sendRecv: ~ forall tn, t1 <= tn < t3 -> (forall m, ~ mark mch p c a tn m) /\
+                                                      (forall m, ~ recv mch c p a tn m)) by (
                                                                                              unfold not; intros exp; assert (t1LtT3: t1 < t3) by omega; pose proof (noChange dt t1LtT3 exp); firstorder).
       assert (noSend: forall tn, t1 <= tn < t3 -> forall m, ~ mark mch p c a tn m) by (
                                                                                        clear cRespResp;
                                                                                        unfold not; intros tn cond m0 msendm0;
                                                                                        assert (tnLeT: tn <= t) by omega;
-                                                                                       assert (one: forall tc', tc' < t1 -> ~ proc mch p c a tc' m0) by (
-                                                                                                                                                         unfold not; intros tc' tc'LtT1 mprocm0;
-                                                                                                                                                         pose proof (procImpMark mprocm0) as [tm [tmLeTc' msend'm0]];
+                                                                                       assert (one: forall tc', tc' < t1 -> ~ recv mch p c a tc' m0) by (
+                                                                                                                                                         unfold not; intros tc' tc'LtT1 mrecvm0;
+                                                                                                                                                         pose proof (recvImpMark mrecvm0) as [tm [tmLeTc' msend'm0]];
                                                                                                                                                          pose proof (uniqMark2 msendm0 msend'm0) as tmEqTc';
                                                                                                                                                          rewrite <- tmEqTc' in *; omega);
-                                                                                       assert (two: forall tp', tp' < tn -> ~ proc mch c p a tp' m) by (
+                                                                                       assert (two: forall tp', tp' < tn -> ~ recv mch c p a tp' m) by (
                                                                                                                                                         unfold not; intros tp' tp'LtTn; assert (tp'LtT3: tp' < t3) by omega; firstorder);
                                                                                        apply (cross t1 tn t1LeT tnLeT m msendm m0 msendm0 one two)).
 
-      destruct (classical (exists tn, tn < t3 /\ t1 <= tn /\ exists m0, proc mch c p a tn m0)) as [ext|noEx].
-      pose proof (maxExists' classical ext) as [tn [cond [[tnLtT3 [m0 mprocm0]] notAfter]]].
+      destruct (classical (exists tn, tn < t3 /\ t1 <= tn /\ exists m0, recv mch c p a tn m0)) as [ext|noEx].
+      pose proof (maxExists' classical ext) as [tn [cond [[tnLtT3 [m0 mrecvm0]] notAfter]]].
       
-      pose proof (procImpMark mprocm0) as [tr [trLeTn msendm0]].
+      pose proof (recvImpMark mrecvm0) as [tr [trLeTn msendm0]].
       assert (opts: tr = t1 \/ tr > t1 \/ tr < t1) by omega.
       destruct opts as [trEqT1 | [trGtT1 | trLtT1]].
       rewrite trEqT1 in *.
       pose proof (uniqMark1 msendm msendm0) as mEqm0.
       rewrite <- mEqm0 in *.
-      generalize neg cond mprocm0; clear; firstorder.
+      generalize neg cond mrecvm0; clear; firstorder.
       assert (tnLeT: tn <= t) by omega.
-      assert (cond2: forall t4, t4 < tn -> ~ proc mch c p a t4 m) by (
+      assert (cond2: forall t4, t4 < tn -> ~ recv mch c p a t4 m) by (
                                                                       intros t4 t4LtTn; assert (t4LtT3: t4 < t3) by omega;
                                                                       generalize neg t4LtT3; clear; firstorder).
-      apply (cRespResp t1 tr tn tnLeT m msendm m0 msendm0 mprocm0 trGtT1 cond2).
-      assert (notty2': ~ exists t'', tr <= t'' < t1 /\ exists m, proc mch p c a t'' m /\ to m >= state c a t1) by (
-                                                                                                                   unfold not; intros [t'' [cond2 [m1 [mprocm1 _]]]];
-                                                                                                                   pose proof (procImpMark mprocm1) as [t5 [t5LeT'' msendm1]];
+      apply (cRespResp t1 tr tn tnLeT m msendm m0 msendm0 mrecvm0 trGtT1 cond2).
+      assert (notty2': ~ exists t'', tr <= t'' < t1 /\ exists m, recv mch p c a t'' m /\ to m >= state c a t1) by (
+                                                                                                                   unfold not; intros [t'' [cond2 [m1 [mrecvm1 _]]]];
+                                                                                                                   pose proof (recvImpMark mrecvm1) as [t5 [t5LeT'' msendm1]];
                                                                                                                    assert (trLeT: tr <= t) by omega;
                                                                                                                    assert (t5LeT: t5 <= t) by omega;
-                                                                                                                   assert (one: forall tc', tc' < tr -> ~ proc mch p c a tc' m1) by (
-                                                                                                                                                                                     unfold not; intros tc' tc'LtTr mproc'm1;
-                                                                                                                                                                                     pose proof (uniqProc2 mprocm1 mproc'm1) as t''EqTc';
+                                                                                                                   assert (one: forall tc', tc' < tr -> ~ recv mch p c a tc' m1) by (
+                                                                                                                                                                                     unfold not; intros tc' tc'LtTr mrecv'm1;
+                                                                                                                                                                                     pose proof (uniqRecv2 mrecvm1 mrecv'm1) as t''EqTc';
                                                                                                                                                                                      rewrite <- t''EqTc' in *;
                                                                                                                                                                                        omega);
-                                                                                                                   assert (two: forall tp', tp' < t5 -> ~ proc mch c p a tp' m0) by (
-                                                                                                                                                                                     unfold not; intros tp' tp'LtT5 mproc'm0;
-                                                                                                                                                                                     pose proof (uniqProc2 mprocm0 mproc'm0) as tnEqTp';
+                                                                                                                   assert (two: forall tp', tp' < t5 -> ~ recv mch c p a tp' m0) by (
+                                                                                                                                                                                     unfold not; intros tp' tp'LtT5 mrecv'm0;
+                                                                                                                                                                                     pose proof (uniqRecv2 mrecvm0 mrecv'm0) as tnEqTp';
                                                                                                                                                                                      rewrite <- tnEqTp' in *; omega);
                                                                                                                    apply (cross tr t5 trLeT t5LeT m0 msendm0 m1 msendm1 one two)).
-      assert (notty2: ~ exists t'', S tr <= t'' < t1 /\ exists m, proc mch p c a t'' m /\ to m >= state c a t1) by (
+      assert (notty2: ~ exists t'', S tr <= t'' < t1 /\ exists m, recv mch p c a t'' m /\ to m >= state c a t1) by (
                                                                                                                     unfold not; intros [t'' [cond1 rest]]; assert (cond2: tr <= t'' < t1) by omega;
                                                                                                                     generalize notty2' cond2 rest; clear; firstorder).
       assert (strLeT1: S tr <= t1) by omega.
@@ -1108,22 +1108,22 @@ Module Final (dt: DataTypes) (ch: ChannelPerAddr dt) (st: Stuff dt ch).
       pose proof (whenChildHighConv t1LtT2 notty) as sST1LeT2.
       assert (trLtT3: tr < t3) by omega.
       assert (noC: forall tn0, S tn <= tn0 < t3 -> (forall m, ~ mark mch p c a tn0 m) /\
-                                                   (forall m, ~ proc mch c p a tn0 m)) by (
+                                                   (forall m, ~ recv mch c p a tn0 m)) by (
                                                                                            intros tn0 cond2;
                                                                                            constructor; [assert (cond3: t1 <= tn0 < t3) by omega; generalize noSend cond3; clear; firstorder|
                                                                                                          assert (cond4: tn < tn0 < t3) by omega; 
                                                                                                            assert (t1LeTn0: t1 <= tn0) by omega; generalize cond4 t1LeTn0 notAfter; clear; firstorder]).
       assert (sTnLtT3: S tn <= t3) by omega.
       pose proof (noChange2 dt sTnLtT3 noC) as dirEq.
-      generalize st1LeTr sST1LeT2 sTnLtT3 dirEq rsendr rprocr msendm msendm0 mprocm0; clear; intros.
+      generalize st1LeTr sST1LeT2 sTnLtT3 dirEq rsendr rrecvr msendm msendm0 mrecvm0; clear; intros.
       pose proof (sendmChange st msendm) as sEqTom.
       pose proof (sendmImpSt msendm) as sGtTom.
-      pose proof (procmChange dt mprocm0) as dSEqTom0.
+      pose proof (recvmChange dt mrecvm0) as dSEqTom0.
       pose proof (sendmChange st msendm0) as sSEqTom0.
-      pose proof (procmCond rprocr) as dLeFromr.
+      pose proof (recvmCond rrecvr) as dLeFromr.
       pose proof (sendmFrom st rsendr) as sEqFromr.
       omega.
-      generalize sendProc noSend noEx; clear; firstorder.
+      generalize sendRecv noSend noEx; clear; firstorder.
     Qed.
 
     Theorem conservative: forall {a t}, dir p c a t >= state c a t.
@@ -1134,9 +1134,9 @@ Module Final (dt: DataTypes) (ch: ChannelPerAddr dt) (st: Stuff dt ch).
     Qed.
 
     Lemma cRespFifo: forall {a t1 t2 t3 m1 m2}, mark mch c p a t1 m1 -> mark mch c p a t2 m2 ->
-                                                proc mch c p a t3 m2 -> t1 < t2 -> (forall t4, t4 < t3 -> ~ proc mch c p a t4 m1) -> False.
+                                                recv mch c p a t3 m2 -> t1 < t2 -> (forall t4, t4 < t3 -> ~ recv mch c p a t4 m1) -> False.
     Proof.
-      intros a t1 t2 t3 m1 m2 sendm1 sendm2 procm2 t1LtT2.
+      intros a t1 t2 t3 m1 m2 sendm1 sendm2 recvm2 t1LtT2.
       pose proof (@mainInd a t3) as [_ [_ [_ last]]].
       specialize (last t1 t2 t3).
       assert (t3LeT3: t3 <= t3) by omega.
@@ -1144,7 +1144,7 @@ Module Final (dt: DataTypes) (ch: ChannelPerAddr dt) (st: Stuff dt ch).
     Qed.
 
     Lemma cross: forall {a t1 t2 m1 m2}, mark mch c p a t1 m1 -> mark mch p c a t2 m2 ->
-                                         (forall t3, t3 < t1 -> ~ proc mch p c a t3 m2) -> (forall t4, t4 < t2 -> ~ proc mch c p a t4 m1) -> False.
+                                         (forall t3, t3 < t1 -> ~ recv mch p c a t3 m2) -> (forall t4, t4 < t2 -> ~ recv mch c p a t4 m1) -> False.
       intros a t1 t2 m1 m2 sendm1 sendm2 one two.
       assert (opts: t1 <= t2 \/ t1 > t2) by omega.
       destruct opts as [t1LeT2 | t2LtT1].
@@ -1157,171 +1157,171 @@ Module Final (dt: DataTypes) (ch: ChannelPerAddr dt) (st: Stuff dt ch).
       apply (sec t1 t2 t1LeT1 t2LeT1 m1 sendm1 m2 sendm2 one two).
     Qed.
 
-    Theorem cReqRespSent: forall {a t1 t2 r}, mark rch p c a t1 r -> proc rch p c a t2 r ->
+    Theorem cReqRespSent: forall {a t1 t2 r}, mark rch p c a t1 r -> recv rch p c a t2 r ->
                                               to r >= state c a t2 -> exists t3, t3 < t2 /\ exists m, mark mch c p a t3 m /\ to m <= to r /\
-                                                                                                      (forall t4, t4 < t1 -> ~ proc mch c p a t4 m).
+                                                                                                      (forall t4, t4 < t1 -> ~ recv mch c p a t4 m).
     Proof.
-      intros a t1 t2 r sendr procr toRGestT2.
+      intros a t1 t2 r sendr recvr toRGestT2.
       destruct (classical (exists t3, t3 < t2 /\ exists m, mark mch c p a t3 m /\ to m <= to r /\ forall t4,
-                                                                                                    t4 < t1 -> ~ proc mch c p a t4 m)) as [easy|hard].
+                                                                                                    t4 < t1 -> ~ recv mch c p a t4 m)) as [easy|hard].
       intuition.
-      pose proof (procImpMark procr) as [t1' [t1LeT2 send'r]].
+      pose proof (recvImpMark recvr) as [t1' [t1LeT2 send'r]].
       pose proof (uniqMark2 sendr send'r) as t1'EqT1.
       rewrite <- t1'EqT1 in *.
       clear t1'EqT1 send'r t1'.
 
-      destruct (classical (exists t, t < t1 /\ ((exists m, proc mch c p a t m) \/
+      destruct (classical (exists t, t < t1 /\ ((exists m, recv mch c p a t m) \/
                                                 (exists m, mark mch p c a t m)))) as [ex | notEx].
-      pose proof (maxExists' classical ex) as [t [tLtT1 [sendOrProc notAfter]]].
+      pose proof (maxExists' classical ex) as [t [tLtT1 [sendOrRecv notAfter]]].
       assert (nothing: forall y, S t <= y < t1 -> (forall m, ~ mark mch p c a y m) /\
-                                                  (forall m, ~ proc mch c p a y m)) by
+                                                  (forall m, ~ recv mch c p a y m)) by
           (intros y cond; assert (cond2: t < y < t1)by omega; generalize cond2 notAfter; clear; firstorder).
       pose proof (noChange2 dt tLtT1 nothing) as dirEq.
       clear nothing.
-      destruct sendOrProc as [[m procm] | [m sendm]].
-      pose proof (procImpMark procm) as [t' [t'LeT sendm]].
-      assert (noCProc: forall tm, t' <= tm < t2 -> forall m', ~ proc mch p c a tm m') by (
-                                                                                          unfold not; intros tm cond m' procm';
-                                                                                          pose proof (procImpMark procm') as [ts [tsLeTm sendm']];
+      destruct sendOrRecv as [[m recvm] | [m sendm]].
+      pose proof (recvImpMark recvm) as [t' [t'LeT sendm]].
+      assert (noCRecv: forall tm, t' <= tm < t2 -> forall m', ~ recv mch p c a tm m') by (
+                                                                                          unfold not; intros tm cond m' recvm';
+                                                                                          pose proof (recvImpMark recvm') as [ts [tsLeTm sendm']];
                                                                                           assert (opts: ts < t \/ ts = t \/ t < ts < t1 \/ t1 <= ts) by omega;
                                                                                           destruct opts as [tsLtT | [tsEqT | [tLtTsLtT1  | t1LeTs ]]]; [
-                                                                                            assert (one: forall x, x < t' -> ~ proc mch p c a x m') by ( unfold not; intros x xLtT' proc'm';
-                                                                                                                                                         pose proof (uniqProc2 procm' proc'm') as xEqTm; omega);
-                                                                                            assert (two: forall x, x < ts -> ~ proc mch c p a x m) by (unfold not; intros x xLtTs proc'm;
-                                                                                                                                                       pose proof (uniqProc2 procm proc'm) as xEqTs; omega);
+                                                                                            assert (one: forall x, x < t' -> ~ recv mch p c a x m') by ( unfold not; intros x xLtT' recv'm';
+                                                                                                                                                         pose proof (uniqRecv2 recvm' recv'm') as xEqTm; omega);
+                                                                                            assert (two: forall x, x < ts -> ~ recv mch c p a x m) by (unfold not; intros x xLtTs recv'm;
+                                                                                                                                                       pose proof (uniqRecv2 recvm recv'm) as xEqTs; omega);
                                                                                             apply (cross sendm sendm' one two) |
                                                                                             rewrite tsEqT in *;
-                                                                                              apply (noSendmProcm dt sendm' procm) |
+                                                                                              apply (noSendmRecvm dt sendm' recvm) |
                                                                                             generalize notAfter tLtTsLtT1 sendm'; clear; firstorder |
-                                                                                            pose proof (pReqResp noTwoPResp noTwoPReqNon sendr sendm' procm' t1LeTs) as [t4 [t4LtTm proc'r]];
-                                                                                              pose proof (uniqProc2 procr proc'r) as t4EqT2; omega]).
+                                                                                            pose proof (pReqResp noTwoPResp noTwoPReqNon sendr sendm' recvm' t1LeTs) as [t4 [t4LtTm recv'r]];
+                                                                                              pose proof (uniqRecv2 recvr recv'r) as t4EqT2; omega]).
       destruct (classical (exists ts, ts < t2 /\ t' < ts /\ exists m', mark mch c p a ts m'))
         as [ ex2 | notEx2].
       pose proof (maxExists' classical ex2) as [ts [tsLtT2 [[t'LtTs [m' sendm']] notAfter2]]].
       assert (nothing: forall y, S ts <= y < t2 ->
-                                 (forall m, ~ mark mch c p a y m) /\ (forall m, ~ proc mch p c a y m)) by
+                                 (forall m, ~ mark mch c p a y m) /\ (forall m, ~ recv mch p c a y m)) by
           (intros y cond; assert (cond1: t' < y < t2) by omega; assert (cond2: t' <= y < t2) by omega;
-           generalize notAfter2 noCProc cond cond1 cond2; clear; firstorder).
+           generalize notAfter2 noCRecv cond cond1 cond2; clear; firstorder).
       pose proof (noChange2 st tsLtT2 nothing) as stEq.
-      destruct (classical (exists tr, tr < t1 /\ proc mch c p a tr m')) as [ [tr [trLtT1 procm']] | noProc].
+      destruct (classical (exists tr, tr < t1 /\ recv mch c p a tr m')) as [ [tr [trLtT1 recvm']] | noRecv].
       assert (opts: tr < t \/ tr = t \/ t < tr < t1) by omega.
       destruct opts as [trLtT | [trEqT | cond]].
-      assert (forall t4, t4 < tr -> ~ proc mch c p a t4 m) by (
-                                                               unfold not; intros t4 t4LtTr proc'm; pose proof (uniqProc2 procm proc'm) as t4EqT; omega).
-      pose proof (cRespFifo sendm sendm' procm' t'LtTs). intuition.
+      assert (forall t4, t4 < tr -> ~ recv mch c p a t4 m) by (
+                                                               unfold not; intros t4 t4LtTr recv'm; pose proof (uniqRecv2 recvm recv'm) as t4EqT; omega).
+      pose proof (cRespFifo sendm sendm' recvm' t'LtTs). intuition.
       rewrite trEqT in *.
-      pose proof (uniqProc1 procm procm') as mEqM'.
+      pose proof (uniqRecv1 recvm recvm') as mEqM'.
       rewrite mEqM' in *.
       pose proof (uniqMark2 sendm sendm') as t'EqTs.
       omega.
-      generalize notAfter cond procm'; clear; firstorder.
+      generalize notAfter cond recvm'; clear; firstorder.
       assert (opts: to m' <= to r \/ to m' > to r) by omega.
       destruct opts as [toM'LeToR | toM'GtToR].
-      generalize tsLtT2 sendm' toM'LeToR noProc; clear; firstorder.
+      generalize tsLtT2 sendm' toM'LeToR noRecv; clear; firstorder.
       pose proof (sendmChange  st sendm') as stEqToM'.
       omega.
       assert (nothing: forall y, S t' <= y < t2 ->
-                                 (forall m, ~ mark mch c p a y m) /\ (forall m, ~ proc mch p c a y m)) by
+                                 (forall m, ~ mark mch c p a y m) /\ (forall m, ~ recv mch p c a y m)) by
           (intros y cond; assert (cond2: t' <= y < t2) by omega;
-           generalize notEx2 noCProc cond cond2; clear; firstorder).
+           generalize notEx2 noCRecv cond cond2; clear; firstorder).
       assert (t'LeT2: S t' <= t2) by omega.
       pose proof (noChange2 st t'LeT2 nothing) as stEq.
       pose proof (sendrImpSt dt sendr) as toRLtD.
       pose proof (sendmChange  st sendm) as st1.
-      pose proof (procmChange dt procm) as st2.
+      pose proof (recvmChange dt recvm) as st2.
       omega.
 
       assert (tLeT1: t <= t1) by omega.
-      pose proof (pRespReq noTwoPResp noTwoPReqNon sendm sendr procr tLeT1) as [t' [t'LtT2 procm]].
-      pose proof (procImpMark procm) as [t'' [tLeT' send'm]].
+      pose proof (pRespReq noTwoPResp noTwoPReqNon sendm sendr recvr tLeT1) as [t' [t'LtT2 recvm]].
+      pose proof (recvImpMark recvm) as [t'' [tLeT' send'm]].
       pose proof (uniqMark2 sendm send'm) as t''EqT.
       rewrite <- t''EqT in *. clear t''EqT t'' send'm.
-      assert (noCProc: forall tm, t' < tm < t2 -> forall m', ~ proc mch p c a tm m').
-      unfold not; intros tm cond m' procm';
-      pose proof (procImpMark procm') as [ts [tsLeTm sendm']];
+      assert (noCRecv: forall tm, t' < tm < t2 -> forall m', ~ recv mch p c a tm m').
+      unfold not; intros tm cond m' recvm';
+      pose proof (recvImpMark recvm') as [ts [tsLeTm sendm']];
       assert (opts: ts < t \/ ts = t \/ t < ts < t1 \/ t1 <= ts) by omega;
       destruct opts as [tsLtT | [tsEqT | [tLtTsLtT1  | t1LeTs ]]]; [
-        pose proof (sendmImpProcr sendm) as [r' procr'];
-        pose proof (procImpMark procr') as [tx [txLeT sendr']];
-        assert (one: forall t3, t3 < tx -> ~ proc mch p c a t3 m') by (
-                                                                       unfold not; intros t3 t3LtTx proc'm'; pose proof (uniqProc2 procm' proc'm') as t3EqTr;
+        pose proof (sendmImpRecvr sendm) as [r' recvr'];
+        pose proof (recvImpMark recvr') as [tx [txLeT sendr']];
+        assert (one: forall t3, t3 < tx -> ~ recv mch p c a t3 m') by (
+                                                                       unfold not; intros t3 t3LtTx recv'm'; pose proof (uniqRecv2 recvm' recv'm') as t3EqTr;
                                                                        omega);
-        assert (two: forall t4, t4 <= ts -> ~ proc rch c p a t4 r') by (
-                                                                        unfold not; intros t4 t4LeTs proc'r'; pose proof (uniqProc2 procr' proc'r') as t4EqTs;
+        assert (two: forall t4, t4 <= ts -> ~ recv rch c p a t4 r') by (
+                                                                        unfold not; intros t4 t4LeTs recv'r'; pose proof (uniqRecv2 recvr' recv'r') as t4EqTs;
                                                                         omega);
         apply (cReqPRespCross sendr' sendm' one two)|
         rewrite tsEqT in *; pose proof (uniqMark1 sendm sendm') as mEqM'; rewrite mEqM' in *;
-        pose proof (uniqProc2 procm procm') as trEqT'; omega |
+        pose proof (uniqRecv2 recvm recvm') as trEqT'; omega |
         generalize notAfter tLtTsLtT1 sendm'; clear; firstorder |
-        pose proof (pReqResp noTwoPResp noTwoPReqNon sendr sendm' procm' t1LeTs) as [t4 [t4LtTm proc'r]];
-          pose proof (uniqProc2 procr proc'r) as t4EqT2; omega].
+        pose proof (pReqResp noTwoPResp noTwoPReqNon sendr sendm' recvm' t1LeTs) as [t4 [t4LtTm recv'r]];
+          pose proof (uniqRecv2 recvr recv'r) as t4EqT2; omega].
       
       destruct (classical (exists ts, ts < t2 /\ t' < ts /\ exists m', mark mch c p a ts m'))
         as [ ex2 | notEx2].
       pose proof (maxExists' classical ex2) as [ts [tsLtT2 [[t'LtTs [m' sendm']] notAfter2]]].
       assert (nothing: forall y, S ts <= y < t2 ->
-                                 (forall m, ~ mark mch c p a y m) /\ (forall m, ~ proc mch p c a y m)) by
+                                 (forall m, ~ mark mch c p a y m) /\ (forall m, ~ recv mch p c a y m)) by
           (intros y cond; assert (cond1: t' < y < t2) by omega;
-           generalize notAfter2 noCProc cond cond1; clear; firstorder).
+           generalize notAfter2 noCRecv cond cond1; clear; firstorder).
       pose proof (noChange2 st tsLtT2 nothing) as stEq.
-      destruct (classical (exists tr, tr < t1 /\ proc mch c p a tr m')) as [ [tr [trLtT1 procm']] | noProc].
-      pose proof (procImpMark procm') as [ts' [ts'LeTr send'm']].
+      destruct (classical (exists tr, tr < t1 /\ recv mch c p a tr m')) as [ [tr [trLtT1 recvm']] | noRecv].
+      pose proof (recvImpMark recvm') as [ts' [ts'LeTr send'm']].
       pose proof (uniqMark2 send'm' sendm') as ts'EqTs.
       assert (trGtT: tr > t) by omega.
       clear ts' ts'LeTr send'm' ts'EqTs.
       assert (opts: t < tr < t1 \/ t1 <= tr) by omega.
       destruct opts as [cond1 | t1LeTr].
-      generalize cond1 notAfter procm'; clear; firstorder.
+      generalize cond1 notAfter recvm'; clear; firstorder.
       assert (opts: to m' <= to r \/ to m' > to r) by omega.
       destruct opts as [toM'LeToR | toM'GtToR].
-      assert (noProc: forall t4, t4 < t1 -> ~ proc mch c p a t4 m') by (
-                                                                        unfold not; intros t4 t4LtT1 proc'm'; pose proof (uniqProc2 procm' proc'm') as t4EqTr; omega).
-      generalize tsLtT2 sendm' toM'LeToR noProc; clear; firstorder.
+      assert (noRecv: forall t4, t4 < t1 -> ~ recv mch c p a t4 m') by (
+                                                                        unfold not; intros t4 t4LtT1 recv'm'; pose proof (uniqRecv2 recvm' recv'm') as t4EqTr; omega).
+      generalize tsLtT2 sendm' toM'LeToR noRecv; clear; firstorder.
       pose proof (sendmChange st sendm') as stEqToM'.
       omega.
-      assert (last: forall t4, t4 < t1 -> ~ proc mch c p a t4 m') by (generalize noProc; clear; firstorder).
+      assert (last: forall t4, t4 < t1 -> ~ recv mch c p a t4 m') by (generalize noRecv; clear; firstorder).
       assert (opts: to m' <= to r \/ to m' > to r) by omega.
       destruct opts as [toM'LeToR | toM'GtToR].
       generalize last tsLtT2 toM'LeToR sendm'; clear; firstorder.
       pose proof (sendmChange st sendm') as stEqToM'.
       omega.
       assert (nothing: forall y, S t' <= y < t2 ->
-                                 (forall m, ~ mark mch c p a y m) /\ (forall m, ~ proc mch p c a y m)) by
-          (generalize noCProc notEx2; clear; firstorder).
+                                 (forall m, ~ mark mch c p a y m) /\ (forall m, ~ recv mch p c a y m)) by
+          (generalize noCRecv notEx2; clear; firstorder).
       pose proof (noChange2 st t'LtT2 nothing) as stEq.
-      pose proof (procmChange st procm) as st1.
+      pose proof (recvmChange st recvm) as st1.
       pose proof (sendmChange dt sendm) as d1.
       pose proof (sendrImpSt dt sendr) as d2.
       omega.
-      assert (cNoProc: forall t4, t4 < t2 -> forall m, ~ proc mch p c a t4 m) by (
-                                                                                  unfold not; intros t4 t4LtT2 m procm; pose proof (procImpMark procm) as [t3 [t3LeT4 sendm]];
+      assert (cNoRecv: forall t4, t4 < t2 -> forall m, ~ recv mch p c a t4 m) by (
+                                                                                  unfold not; intros t4 t4LtT2 m recvm; pose proof (recvImpMark recvm) as [t3 [t3LeT4 sendm]];
                                                                                   assert (opts: t3 < t1 \/ t3 >= t1) by omega;
                                                                                   destruct opts as [t3LtT1 | t4GeT1]; [
                                                                                     generalize notEx t3LtT1 sendm; clear; firstorder;
                                                                                     intuition |
-                                                                                    pose proof (pReqResp noTwoPResp noTwoPReqNon sendr sendm procm t4GeT1) as [t5 [t4LtT4 proc'r]];
-                                                                                      pose proof (uniqProc2 procr proc'r) as t5EqT2; omega]).
+                                                                                    pose proof (pReqResp noTwoPResp noTwoPReqNon sendr sendm recvm t4GeT1) as [t5 [t4LtT4 recv'r]];
+                                                                                      pose proof (uniqRecv2 recvr recv'r) as t5EqT2; omega]).
       destruct (classical (exists t3, t3 < t2 /\ exists m, mark mch c p a t3 m)) as [ex2 | notEx2].
       pose proof (maxExists' classical ex2) as [ts [tsLtT2 [[m' sendm'] notAfter2]]].
       assert (nothing: forall y, S ts <= y < t2 ->
-                                 (forall m, ~ mark mch c p a y m) /\ (forall m, ~ proc mch p c a y m)) by
+                                 (forall m, ~ mark mch c p a y m) /\ (forall m, ~ recv mch p c a y m)) by
           (intros y cond;
-           generalize notAfter2 cNoProc cond; clear; firstorder).
+           generalize notAfter2 cNoRecv cond; clear; firstorder).
       pose proof (noChange2 st tsLtT2 nothing) as stEq.
-      destruct (classical (exists tr, tr < t1 /\ proc mch c p a tr m')) as [ [tr [trLtT1 procm']] | noProc].
-      generalize notEx trLtT1 procm'; clear; firstorder.
+      destruct (classical (exists tr, tr < t1 /\ recv mch c p a tr m')) as [ [tr [trLtT1 recvm']] | noRecv].
+      generalize notEx trLtT1 recvm'; clear; firstorder.
       assert (opts: to m' <= to r \/ to m' > to r) by omega.
       destruct opts as [toM'LeToR | toM'GtToR].
-      generalize toM'LeToR noProc tsLtT2 sendm'; clear; firstorder.
+      generalize toM'LeToR noRecv tsLtT2 sendm'; clear; firstorder.
       pose proof (sendmChange st sendm') as stEqToM'.
       omega.
       assert (nothing1: forall y, 0 <= y < t2 ->
-                                  (forall m, ~ mark mch c p a y m) /\ (forall m, ~ proc mch p c a y m)) by
-          (generalize cNoProc notEx2; clear; firstorder).
+                                  (forall m, ~ mark mch c p a y m) /\ (forall m, ~ recv mch p c a y m)) by
+          (generalize cNoRecv notEx2; clear; firstorder).
       assert (x1: 0 <= t2) by omega.
       pose proof (noChange2 st x1 nothing1) as st1.
       assert (nothing2: forall y, 0 <= y < t1 ->
-                                  (forall m, ~ mark mch p c a y m) /\ (forall m, ~ proc mch c p a y m)) by
+                                  (forall m, ~ mark mch p c a y m) /\ (forall m, ~ recv mch c p a y m)) by
           (generalize notEx; clear; firstorder).
       assert (x2: 0 <= t1) by omega.
       pose proof (noChange2 dt x2 nothing2) as d1.
@@ -1332,36 +1332,36 @@ Module Final (dt: DataTypes) (ch: ChannelPerAddr dt) (st: Stuff dt ch).
 
     Lemma vol: forall {a t}, forall {t1 r1}, mark rch p c a t1 r1 ->
                                              forall {t2 m2}, mark mch c p a t2 m2 ->
-                                                             forall {t3}, t3 <= t -> t1 <= t3 -> proc mch c p a t3 m2 ->
-                                                                          (forall {t4}, t4 <= t2 -> ~ proc rch p c a t4 r1) ->
+                                                             forall {t3}, t3 <= t -> t1 <= t3 -> recv mch c p a t3 m2 ->
+                                                                          (forall {t4}, t4 <= t2 -> ~ recv rch p c a t4 r1) ->
                                                                           (forall {t5}, t1 < t5 <= t3 -> forall r, ~ mark rch p c a t5 r) ->
-                                                                          forall r3, proc rch p c a t2 r3 -> to r3 < state c a t2 -> False.
+                                                                          forall r3, recv rch p c a t2 r3 -> to r3 < state c a t2 -> False.
     Proof.
       intros a.
       induction t.
-      intros t1 r1 sendr1 t2 m2 sendm2 t3 t3LeT t1LeT3 procm2 notProcr1 notSendr r3
-             procr3 toR3LtStT2.
+      intros t1 r1 sendr1 t2 m2 sendm2 t3 t3LeT t1LeT3 recvm2 notRecvr1 notSendr r3
+             recvr3 toR3LtStT2.
       unfold Time in *.
-      pose proof (ch.procImpMark procm2) as [t' [t'LeT3 send'm2]].
+      pose proof (ch.recvImpMark recvm2) as [t' [t'LeT3 send'm2]].
       pose proof (ch.uniqMark2 sendm2 send'm2) as t'EqT2.
       assert (t3Eq0: t3 = 0) by omega.
       assert (t2Eq0: t2 = 0) by omega.
       assert (t1Eq0: t1 = 0) by omega.
       rewrite t3Eq0, t2Eq0, t1Eq0 in *; clear t' t'LeT3 send'm2 t'EqT2 t1Eq0
                                               t2Eq0 t3Eq0 t3LeT t1LeT3.
-      pose proof (ch.procImpMark procr3) as [t' [t'Le0 send'r3]].
+      pose proof (ch.recvImpMark recvr3) as [t' [t'Le0 send'r3]].
       assert (t'Eq0: t' = 0) by omega; rewrite t'Eq0 in *.
       pose proof (ch.uniqMark1 sendr1 send'r3) as r1EqR3.
       rewrite r1EqR3 in *.
       firstorder.
 
-      intros t1 r1 sendr1 t2 m2 sendm2 t3 t3LeT t1LeT3 procm2 notProcr1 notSendr r3
-             procr3 toR3LtStT2.
+      intros t1 r1 sendr1 t2 m2 sendm2 t3 t3LeT t1LeT3 recvm2 notRecvr1 notSendr r3
+             recvr3 toR3LtStT2.
       unfold Time in *.
-      pose proof (ch.procImpMark procm2) as [t' [t2LeT3 send'm2]].
+      pose proof (ch.recvImpMark recvm2) as [t' [t2LeT3 send'm2]].
       pose proof (ch.uniqMark2 sendm2 send'm2) as t'EqT2.
       rewrite <- t'EqT2 in *; clear send'm2 t' t'EqT2.
-      pose proof (ch.procImpMark procr3) as [ts [tsLeT2 sendr3]].
+      pose proof (ch.recvImpMark recvr3) as [ts [tsLeT2 sendr3]].
       assert (opts: ts > t3 \/ t1 < ts <= t3 \/ ts = t1 \/ ts < t1) by omega.
       destruct opts as [tsGtT3 | [cond | [tsEqT1 | tsLtT1]]].
       omega.
@@ -1369,7 +1369,7 @@ Module Final (dt: DataTypes) (ch: ChannelPerAddr dt) (st: Stuff dt ch).
       assert (t2LeT2: t2 <= t2) by omega.
       rewrite tsEqT1 in *. pose proof (ch.uniqMark1 sendr3 sendr1) as r1EqR3.
       rewrite r1EqR3 in *.
-      generalize notProcr1 t2LeT2 procr3; clear; firstorder.
+      generalize notRecvr1 t2LeT2 recvr3; clear; firstorder.
       pose proof (sendrImpNoSendr dt tsLtT1 sendr3 sendr1) as exist. 
       destruct exist as [tx [cond dirLt']].
       (*    pose proof (minExists classical exist) as [tx [[cond dirLt'] notBefore]]. *)
@@ -1377,60 +1377,60 @@ Module Final (dt: DataTypes) (ch: ChannelPerAddr dt) (st: Stuff dt ch).
       pose proof (sendrImpSt dt sendr3) as gt.
       assert (dirGt: dir p c a ts > dir p c a tx) by omega.
       destruct (classical (exists tn, ts <= tn < tx /\ ((exists m, mark mch p c a tn m) \/
-                                                        (exists m, proc mch c p a tn m /\ to m <= to r3)))) as [sth|notExist].
-      destruct (minExists classical sth) as [tn [[cond2 sendOrProc] notBefore]].
-      (* destruct sth as [tn [cond2 sendOrProc]]. *)
-      destruct sendOrProc as [[m sendm] | [m [procm toMLeToR3]]].
+                                                        (exists m, recv mch c p a tn m /\ to m <= to r3)))) as [sth|notExist].
+      destruct (minExists classical sth) as [tn [[cond2 sendOrRecv] notBefore]].
+      (* destruct sth as [tn [cond2 sendOrRecv]]. *)
+      destruct sendOrRecv as [[m sendm] | [m [recvm toMLeToR3]]].
       assert (opts: ts = tn \/ ts < tn) by omega.
       destruct opts as [tsEqTn | tsLtTn].
       rewrite tsEqTn in *.
       apply (noSendmSendr dt sendm sendr3).
-      pose proof (sendrImpNoSendm tsLtTn sendr3 sendm) as [t' [cond3 [m' [procm' toM'LeToR3]]]].
+      pose proof (sendrImpNoSendm tsLtTn sendr3 sendm) as [t' [cond3 [m' [recvm' toM'LeToR3]]]].
       assert (cond4: ts <= t' < tx) by omega.
       assert (cond5: t' < tn) by omega.
-      generalize notBefore procm' toM'LeToR3 cond4 cond5; clear; firstorder.
-      pose proof (ch.procImpMark procm) as [t'' [t''Letn sendm]].
+      generalize notBefore recvm' toM'LeToR3 cond4 cond5; clear; firstorder.
+      pose proof (ch.recvImpMark recvm) as [t'' [t''Letn sendm]].
       assert (opts: t'' > t2 \/ t'' = t2 \/ t'' < t2) by omega.
       destruct opts as [t''GtT2 | [t''EqT2 | t''LtT2]].
-      assert (notProc: forall tq, tq < tn -> ~ proc mch c p a tq m2) by (
-                                                                         unfold not; intros tq tqLtTn procq;
-                                                                         pose proof (ch.uniqProc2 procq procm2) as tqEqT'';
+      assert (notRecv: forall tq, tq < tn -> ~ recv mch c p a tq m2) by (
+                                                                         unfold not; intros tq tqLtTn recvq;
+                                                                         pose proof (ch.uniqRecv2 recvq recvm2) as tqEqT'';
                                                                          omega).
-      apply (cRespFifo sendm2 sendm procm t''GtT2 notProc).
+      apply (cRespFifo sendm2 sendm recvm t''GtT2 notRecv).
       rewrite t''EqT2 in *.
       pose proof (ch.uniqMark1 sendm sendm2) as mEqM2.
       rewrite mEqM2 in *.
-      pose proof (ch.uniqProc2 procm procm2) as t3EqTn.
+      pose proof (ch.uniqRecv2 recvm recvm2) as t3EqTn.
       omega.
-      assert (nothing: forall ty, t'' <= ty < t2 -> forall q, ~ proc mch p c a ty q).
-      unfold not; intros ty cond3 q procq.
+      assert (nothing: forall ty, t'' <= ty < t2 -> forall q, ~ recv mch p c a ty q).
+      unfold not; intros ty cond3 q recvq.
       assert (opts: t'' = ty \/ t'' < ty) by omega.
       destruct opts as [t''EqTy | t''LtTy].
       rewrite t''EqTy in *.
-      apply (noSendmProcm st sendm procq).
-      pose proof (ch.procImpMark procq) as [tz [tzLeTy sendq]].
+      apply (noSendmRecvm st sendm recvq).
+      pose proof (ch.recvImpMark recvq) as [tz [tzLeTy sendq]].
       assert (opts: tz < ts \/ tz = ts \/ tz > ts) by omega.
       destruct opts as [tzLtTs | [tzEqTs | tzGtTs]].
       assert (tzLtT1: tz < t1) by omega.
-      assert (one: forall t0, t0 < t'' -> ~ proc mch p c a t0 q) by (
-                                                                     unfold not; intros t0 t0LtT'' proc'q;
-                                                                     pose proof (ch.uniqProc2 procq proc'q) as t0EqTz;
+      assert (one: forall t0, t0 < t'' -> ~ recv mch p c a t0 q) by (
+                                                                     unfold not; intros t0 t0LtT'' recv'q;
+                                                                     pose proof (ch.uniqRecv2 recvq recv'q) as t0EqTz;
                                                                      omega).
-      assert (two: forall t0, t0 < tz -> ~ proc mch c p a t0 m) by (
-                                                                    unfold not; intros t0 t0LtTz proc'm;
-                                                                    pose proof (ch.uniqProc2 procm proc'm); omega).
+      assert (two: forall t0, t0 < tz -> ~ recv mch c p a t0 m) by (
+                                                                    unfold not; intros t0 t0LtTz recv'm;
+                                                                    pose proof (ch.uniqRecv2 recvm recv'm); omega).
       apply (cross sendm sendq one two).
       rewrite tzEqTs in *.
       apply (noSendmSendr dt sendq sendr3).
       pose proof @pReqResp.
       assert (tsLeTz: ts <= tz) by omega.
-      pose proof (pReqResp noTwoPResp noTwoPReqNon sendr3 sendq procq tsLeTz) as sth2.
-      destruct sth2 as [t4 [t4LtTy proc'r3]].
-      pose proof (ch.uniqProc2 procr3 proc'r3); omega.
-      assert (nothing2: forall ty, S t'' <= ty < t2 -> forall q, ~ proc mch p c a ty q) by (
+      pose proof (pReqResp noTwoPResp noTwoPReqNon sendr3 sendq recvq tsLeTz) as sth2.
+      destruct sth2 as [t4 [t4LtTy recv'r3]].
+      pose proof (ch.uniqRecv2 recvr3 recv'r3); omega.
+      assert (nothing2: forall ty, S t'' <= ty < t2 -> forall q, ~ recv mch p c a ty q) by (
                                                                                             intros ty cond4; assert (h: t'' <= ty < t2) by omega; generalize h nothing; clear;
                                                                                             firstorder).
-      assert (nothing3: ~ exists ty, S t'' <= ty < t2 /\ exists q, proc mch p c a ty q /\
+      assert (nothing3: ~ exists ty, S t'' <= ty < t2 /\ exists q, recv mch p c a ty q /\
                                                                    to q >= state c a t2) by (generalize nothing2; clear; firstorder).
       pose proof (whenChildHighConv t''LtT2 nothing3) as stLe.
       assert (contra: ~ exists tk, tk < tn /\ ts <= tk /\ exists m, mark mch p c a tk m) by (
@@ -1441,10 +1441,10 @@ Module Final (dt: DataTypes) (ch: ChannelPerAddr dt) (st: Stuff dt ch).
                                                           pose proof (whenDirLow tsLeTn sttt) as sth3; generalize contra sth3; clear; firstorder).
       assert (good: dir p c a tn <= dir p c a ts) by omega.
       pose proof (sendmChange st sendm) as eq1.
-      pose proof (procmChange dt procm) as eq2.
+      pose proof (recvmChange dt recvm) as eq2.
       pose proof (sendmImpSt sendm) as eq3.
       pose proof (sendmFrom st sendm) as eq4.
-      pose proof (procmCond procm) as eq5.
+      pose proof (recvmCond recvm) as eq5.
       omega.
       assert (tsLeTx: ts <= tx) by omega.
       pose proof (sendrFrom dt sendr3).
@@ -1458,12 +1458,12 @@ Module Final (dt: DataTypes) (ch: ChannelPerAddr dt) (st: Stuff dt ch).
                                                         mark rch p c a t2 r2 -> t1 < t2 ->
                                                         (forall ts, t1 < ts < t2 -> forall r, ~ mark rch p c a ts r) ->
                                                         (forall ts, t1 < ts < t2 -> forall m, ~ mark mch p c a ts m) ->
-                                                        (forall t3, t3 <= t -> ~ proc rch p c a t3 r1) ->
-                                                        (forall t4, t4 <= t -> ~ proc rch p c a t4 r2) -> exists t5 m, mark mch c p a t5 m /\
-                                                                                                                       exists t6, t1 <= t6 < t2 /\ proc mch c p a t6 m /\ 
-                                                                                                                                  (forall r, proc rch p c a t5 r -> to r >= state c a t5) /\ to r2 < to m.
+                                                        (forall t3, t3 <= t -> ~ recv rch p c a t3 r1) ->
+                                                        (forall t4, t4 <= t -> ~ recv rch p c a t4 r2) -> exists t5 m, mark mch c p a t5 m /\
+                                                                                                                       exists t6, t1 <= t6 < t2 /\ recv mch c p a t6 m /\ 
+                                                                                                                                  (forall r, recv rch p c a t5 r -> to r >= state c a t5) /\ to r2 < to m.
     Proof.
-      intros t a t1 t2 r1 r2 t1LeT t2LeT sendr1 sendr2 t1LtT2 noSendR noSendM noProcR1 noProcR2.
+      intros t a t1 t2 r1 r2 t1LeT t2LeT sendr1 sendr2 t1LtT2 noSendR noSendM noRecvR1 noRecvR2.
       pose proof (sendrImpNoSendr dt t1LtT2 sendr1 sendr2) as ex1.
       assert (ex2: exists t', t' <= t2 /\ t1 < t' /\ ~ lt (to r1) (dir p c a t')) by
           firstorder.
@@ -1471,9 +1471,9 @@ Module Final (dt: DataTypes) (ch: ChannelPerAddr dt) (st: Stuff dt ch).
       pose proof (sendrImpSt dt sendr1) as dirSth.
       assert (dirNotEq: dir p c a t' <> dir p c a t1) by omega.
       destruct (classical (exists tn, tn < t' /\ t1 <= tn /\ ((exists m, mark mch p c a tn m) \/
-                                                              exists m, proc mch c p a tn m))) as [ext|easy].
-      pose proof (maxExists' classical ext) as [tn [tnLtT'[[t1LeTn sendOrProc] notAfter]]].
-      destruct sendOrProc as [[m sendm] | [m procm]].
+                                                              exists m, recv mch c p a tn m))) as [ext|easy].
+      pose proof (maxExists' classical ext) as [tn [tnLtT'[[t1LeTn sendOrRecv] notAfter]]].
+      destruct sendOrRecv as [[m sendm] | [m recvm]].
       unfold Time in *.
       assert (opts: t1 = tn \/ t1 < tn) by omega.
       destruct opts as [t1EqTn | t1LtTn].
@@ -1482,20 +1482,20 @@ Module Final (dt: DataTypes) (ch: ChannelPerAddr dt) (st: Stuff dt ch).
       assert (tnLtT2: tn < t2) by omega.
       generalize noSendM t1LtTn tnLtT2 sendm; clear; firstorder.
       assert (tnLeTn: tn <= tn) by omega.
-      pose proof (ch.procImpMark procm) as [tm [tmLeTn sendm]].
-      assert (noProc'R1: forall t4, t4 <= tm -> ~ proc rch p c a t4 r1) by (
-                                                                            unfold not; intros t4 cond4 procr1; assert (sth: t4 <= t) by omega;
-                                                                            generalize noProcR1 sth procr1; clear; firstorder).
+      pose proof (ch.recvImpMark recvm) as [tm [tmLeTn sendm]].
+      assert (noRecv'R1: forall t4, t4 <= tm -> ~ recv rch p c a t4 r1) by (
+                                                                            unfold not; intros t4 cond4 recvr1; assert (sth: t4 <= t) by omega;
+                                                                            generalize noRecvR1 sth recvr1; clear; firstorder).
       assert (noSendAny: forall t5, t1 < t5 <= tn -> forall r, ~ mark rch p c a t5 r) by (
                                                                                           intros t5 cond4; assert (sth: t1 < t5 < t2) by omega; generalize noSendR sth;
                                                                                           clear; firstorder).
-      pose proof (vol sendr1 sendm tnLeTn t1LeTn procm noProc'R1 noSendAny) as isVol.
-      assert (isVolR: forall r3, proc rch p c a tm r3 -> to r3 >= state c a tm) by (
-                                                                                    intros r3 proc'r3; specialize (isVol r3 proc'r3); omega).
+      pose proof (vol sendr1 sendm tnLeTn t1LeTn recvm noRecv'R1 noSendAny) as isVol.
+      assert (isVolR: forall r3, recv rch p c a tm r3 -> to r3 >= state c a tm) by (
+                                                                                    intros r3 recv'r3; specialize (isVol r3 recv'r3); omega).
       assert (cond3: t1 <= tn < t2) by omega.
       assert (StnLeT': S tn <= t') by omega.
       assert (noChange: forall tx, S tn <= tx < t' -> (forall m, ~ mark mch p c a tx m) /\
-                                                      forall m, ~ proc mch c p a tx m) by (intros tx cond2;
+                                                      forall m, ~ recv mch c p a tx m) by (intros tx cond2;
                                                                                            assert (cond4: tn < tx < t') by omega; assert (cond6: t1 <= tx) by omega;
                                                                                            generalize notAfter cond4 cond6; clear; firstorder).
       pose proof (noChange2 dt StnLeT' noChange) as dirEq1.
@@ -1504,22 +1504,22 @@ Module Final (dt: DataTypes) (ch: ChannelPerAddr dt) (st: Stuff dt ch).
                                                          pose proof (whenDirLow t'LeT1 d) as [t'' [cond rest]];
                                                          assert (condn: t1 < t'' < t2) by omega; generalize noSendM condn rest; clear; firstorder).
       assert (real: dir p c a t2 <= dir p c a t') by omega.
-      pose proof (procmChange dt procm) as eq1.
+      pose proof (recvmChange dt recvm) as eq1.
       pose proof (sendrImpSt dt sendr2) as eq2.
       assert (H: to r2 < to m) by omega.
-      generalize sendm cond3 procm isVolR H; clear; firstorder.
+      generalize sendm cond3 recvm isVolR H; clear; firstorder.
       assert (Hik: forall tn, t1 <= tn < t' -> (forall m, ~ mark mch p c a tn m) /\
-                                               (forall m, ~ proc mch c p a tn m)) by (generalize easy; clear; firstorder).
+                                               (forall m, ~ recv mch c p a tn m)) by (generalize easy; clear; firstorder).
       pose proof (noChange dt t1LtT' Hik).
       omega.
     Qed.
 
     Theorem pRecvRespPrevState:
-      forall {m a tr ts}, proc mch c p a tr m -> mark mch c p a ts m ->
+      forall {m a tr ts}, recv mch c p a tr m -> mark mch c p a ts m ->
                           dir p c a tr = state c a ts.
     Proof.
       intros.
-      pose proof (procmCond H).
+      pose proof (recvmCond H).
       pose proof (sendmFrom st H0).
       rewrite H1 in H2.
       assumption.
@@ -1527,31 +1527,31 @@ Module Final (dt: DataTypes) (ch: ChannelPerAddr dt) (st: Stuff dt ch).
 
     Theorem noPRespImpSameState:
       forall {sm rm m a},
-        proc mch p c a rm m -> mark mch p c a sm m ->
-        (forall ti mi, ti < sm -> ~ proc mch c p a ti mi /\ ~ mark mch p c a ti mi) ->
+        recv mch p c a rm m -> mark mch p c a sm m ->
+        (forall ti mi, ti < sm -> ~ recv mch c p a ti mi /\ ~ mark mch p c a ti mi) ->
         state c a rm = dir p c a sm.
-      intros sm rm m a procm markm noRecvSend.
-      assert (noCRecv: forall t mt, 0 <= t < rm -> ~ proc mch p c a t mt).
-      unfold not; intros t mt t_lt_rm procmt.
-      pose proof (procImpMark procmt) as [t' [t'_le_t markmt]].
+      intros sm rm m a recvm markm noRecvSend.
+      assert (noCRecv: forall t mt, 0 <= t < rm -> ~ recv mch p c a t mt).
+      unfold not; intros t mt t_lt_rm recvmt.
+      pose proof (recvImpMark recvmt) as [t' [t'_le_t markmt]].
       assert (stuff: t' < sm \/ t' = sm \/ sm < t') by omega.
       destruct stuff as [t'_lt_sm | [t'_eq_sm | sm_lt_t']].
       generalize noRecvSend t'_lt_sm markmt; clear; firstorder.
       rewrite t'_eq_sm in *.
       pose proof (uniqMark1 markm markmt) as m_eq_mt.
       rewrite m_eq_mt in *.
-      pose proof (uniqProc2 procm procmt) as t_eq_rm.
+      pose proof (uniqRecv2 recvm recvmt) as t_eq_rm.
       omega.
-      pose proof (pRespFifo sm_lt_t' markm markmt procmt) as [t'' [t''_lt_t proc'm]].
-      pose proof (uniqProc2 procm proc'm) as t''_eq_rm.
+      pose proof (pRespFifo sm_lt_t' markm markmt recvmt) as [t'' [t''_lt_t recv'm]].
+      pose proof (uniqRecv2 recvm recv'm) as t''_eq_rm.
       omega.
       assert (noCSend: forall t mt, 0 <= t < rm -> ~ mark mch c p a t mt).
       unfold not; intros t mt t_lt_rm markmt.
-      assert (noRecvEarlier: forall ti, ti < sm -> ~ proc mch c p a ti mt) by
+      assert (noRecvEarlier: forall ti, ti < sm -> ~ recv mch c p a ti mt) by
           (generalize noRecvSend; clear; firstorder).
-      assert (noRecvEarlier': forall ti, ti < t -> ~ proc mch p c a ti m) by
-          (unfold not; intros ti ti_lt_t proc'm;
-           pose proof (uniqProc2 procm proc'm) as ti_eq_rm; omega).
+      assert (noRecvEarlier': forall ti, ti < t -> ~ recv mch p c a ti m) by
+          (unfold not; intros ti ti_lt_t recv'm;
+           pose proof (uniqRecv2 recvm recv'm) as ti_eq_rm; omega).
       apply (cross markmt markm noRecvEarlier' noRecvEarlier).
       assert (z_le_sm: 0 <= sm) by omega.
       assert (z_le_rm: 0 <= rm) by omega.
@@ -1565,19 +1565,19 @@ Module Final (dt: DataTypes) (ch: ChannelPerAddr dt) (st: Stuff dt ch).
 
     Theorem noCRespImpSameState:
       forall {sm rm m a},
-        proc mch p c a rm m -> mark mch p c a sm m ->
-        (forall ti mi, ti < rm -> ~ proc mch p c a ti mi /\ ~ mark mch c p a ti mi) ->
+        recv mch p c a rm m -> mark mch p c a sm m ->
+        (forall ti mi, ti < rm -> ~ recv mch p c a ti mi /\ ~ mark mch c p a ti mi) ->
         state c a rm = dir p c a sm.
-      intros sm rm m a procm markm noRecvSend.
-      assert (noPRecv: forall t mt, 0 <= t < sm -> ~ proc mch c p a t mt).
-      unfold not; intros t mt t_lt_sm procmt.
-      pose proof (procImpMark procmt) as [t' [t'_le_t markmt]].
-      pose proof (procImpMarkBefore procm markm) as sm_le_rm.
+      intros sm rm m a recvm markm noRecvSend.
+      assert (noPRecv: forall t mt, 0 <= t < sm -> ~ recv mch c p a t mt).
+      unfold not; intros t mt t_lt_sm recvmt.
+      pose proof (recvImpMark recvmt) as [t' [t'_le_t markmt]].
+      pose proof (recvImpMarkBefore recvm markm) as sm_le_rm.
       assert (t'_lt_rm: t' < rm) by omega.
       generalize noRecvSend t'_lt_rm markmt; clear; firstorder.
       assert (noPSend: forall t mt, t < sm -> ~ mark mch p c a t mt).
       unfold not; intros t mt t_lt_sm markmt.
-      pose proof (pRespFifo t_lt_sm markmt markm procm) as stf.
+      pose proof (pRespFifo t_lt_sm markmt markm recvm) as stf.
       generalize noRecvSend stf; clear; firstorder.
       assert (z_le_sm: 0 <= sm) by omega.
       assert (z_le_rm: 0 <= rm) by omega.
@@ -1590,109 +1590,109 @@ Module Final (dt: DataTypes) (ch: ChannelPerAddr dt) (st: Stuff dt ch).
     Qed.
 
     Theorem cRecvRespPrevState:
-      forall {m a tr ts}, proc mch p c a tr m -> mark mch p c a ts m ->
+      forall {m a tr ts}, recv mch p c a tr m -> mark mch p c a ts m ->
                           state c a tr = dir p c a ts.
     Proof.
-      intros m a tr ts procm markm.
-      pose proof (procImpMarkBefore procm markm) as ts_le_tr.
-      destruct (classical (exists tm', tm' < tr /\ exists mm', proc mch p c a tm' mm'
+      intros m a tr ts recvm markm.
+      pose proof (recvImpMarkBefore recvm markm) as ts_le_tr.
+      destruct (classical (exists tm', tm' < tr /\ exists mm', recv mch p c a tm' mm'
                                                                \/ mark mch c p a tm' mm')) as
           [ex | notEx].
-      pose proof (maxExists' classical ex) as [tm [tm_lt_tr [[mm procm_recvm_mm] notAfter]]].
+      pose proof (maxExists' classical ex) as [tm [tm_lt_tr [[mm recvm_recvm_mm] notAfter]]].
       assert (none: forall y,
                       S tm <= y < tr ->
-                      (forall mm', ~ mark mch c p a y mm') /\ forall mm', ~ proc mch p c a y mm') by
+                      (forall mm', ~ mark mch c p a y mm') /\ forall mm', ~ recv mch p c a y mm') by
           (generalize notAfter; clear; firstorder).
       pose proof noChange2 st tm_lt_tr none as dir_S_tm_eq_dir_ts.
       clear none.
-      destruct procm_recvm_mm as [procm_mm|markm_mm].
-      pose proof procImpMark procm_mm as [tn [tn_le_tm markm_mm]].
-      destruct (classical (exists tk, tn < tk < ts /\ exists mk, proc mch c p a tk mk))
-        as [[tk [tn_le_tk_lt_ts [mk procm_mk]]]|notRecv].
-      pose proof procImpMark procm_mk as [t2 [t2_le_tk markm_mk]].
+      destruct recvm_recvm_mm as [recvm_mm|markm_mm].
+      pose proof recvImpMark recvm_mm as [tn [tn_le_tm markm_mm]].
+      destruct (classical (exists tk, tn < tk < ts /\ exists mk, recv mch c p a tk mk))
+        as [[tk [tn_le_tk_lt_ts [mk recvm_mk]]]|notRecv].
+      pose proof recvImpMark recvm_mk as [t2 [t2_le_tk markm_mk]].
       assert (t2_lt_tr: t2 < tr) by omega.
-      assert (noProc: forall t4, t4 < tn -> ~ proc mch c p a t4 mk) by (
-                                                                        unfold not; intros t4 t4_lt_tn procm_mk'; pose proof (uniqProc2 procm_mk procm_mk');
+      assert (noRecv: forall t4, t4 < tn -> ~ recv mch c p a t4 mk) by (
+                                                                        unfold not; intros t4 t4_lt_tn recvm_mk'; pose proof (uniqRecv2 recvm_mk recvm_mk');
                                                                         omega).
       assert (t2_le_tm: tm < t2 -> False) by (intros l1; generalize notAfter t2_lt_tr l1 markm_mk; clear; firstorder).
-      assert (t2_ne_tm: t2 = tm -> False) by (intro r; rewrite r in *; apply (noSendmProcm st markm_mk procm_mm)).
+      assert (t2_ne_tm: t2 = tm -> False) by (intro r; rewrite r in *; apply (noSendmRecvm st markm_mk recvm_mm)).
       assert (t2_lt_tm: t2 < tm) by omega.
-      assert (noProc': forall t3, t3 < t2 -> ~ proc mch p c a t3 mm) by (
-                                                                         unfold not; intros t3 t3_lt_t2 procm_mm'; pose proof (uniqProc2 procm_mm procm_mm');
+      assert (noRecv': forall t3, t3 < t2 -> ~ recv mch p c a t3 mm) by (
+                                                                         unfold not; intros t3 t3_lt_t2 recvm_mm'; pose proof (uniqRecv2 recvm_mm recvm_mm');
                                                                          omega).
-      pose proof (cross markm_mk markm_mm noProc' noProc); firstorder.
+      pose proof (cross markm_mk markm_mm noRecv' noRecv); firstorder.
       destruct (classical (exists tk, tn < tk < ts /\ exists mk, mark mch p c a tk mk)) as
           [[tk [[tn_lt_tk tk_lt_ts] [mk markm_mk]]] | notSend].
-      pose proof (pRespFifo tk_lt_ts markm_mk markm procm) as [tl [tl_lt_tr procmk]].
-      pose proof (pRespFifo tn_lt_tk markm_mm markm_mk procmk) as [t' [t'_lt_tl proc'mm]].
-      pose proof (uniqProc2 procm_mm proc'mm) as tm_eq_t'.
+      pose proof (pRespFifo tk_lt_ts markm_mk markm recvm) as [tl [tl_lt_tr recvmk]].
+      pose proof (pRespFifo tn_lt_tk markm_mm markm_mk recvmk) as [t' [t'_lt_tl recv'mm]].
+      pose proof (uniqRecv2 recvm_mm recv'mm) as tm_eq_t'.
       rewrite <- tm_eq_t' in *.
-      generalize notAfter tl_lt_tr t'_lt_tl procmk; clear; firstorder.
+      generalize notAfter tl_lt_tr t'_lt_tl recvmk; clear; firstorder.
       assert (st: tn = ts \/ tn > ts \/ tn < ts) by omega.
       destruct st as [eq|[gt|ltt]].
       rewrite eq in *.
       pose proof (uniqMark1 markm_mm markm) as m_eq_mm.
       rewrite m_eq_mm in *.
-      pose proof (uniqProc2 procm procm_mm) as tr_eq_tm.
+      pose proof (uniqRecv2 recvm recvm_mm) as tr_eq_tm.
       omega.
-      pose proof (pRespFifo gt markm markm_mm procm_mm) as [tr1 [tr1_lt_tm proc'm]].
-      pose proof (uniqProc2 procm proc'm) as tr1_eq_tr.
+      pose proof (pRespFifo gt markm markm_mm recvm_mm) as [tr1 [tr1_lt_tm recv'm]].
+      pose proof (uniqRecv2 recvm recv'm) as tr1_eq_tr.
       omega.
       assert (stEq: state c a (S tm) = state c a tr) by
           ( generalize (@noChange2 (state c) gt c p st a (S tm) tr tm_lt_tr) notAfter; clear; firstorder).
       assert (dirEq: dir p c a (S tn) = dir p c a ts) by
           ( generalize (@noChange2 (dir p c) lt p c dt a (S tn) ts ltt) notSend notRecv; clear; firstorder).
-      pose proof (procmChange st procm_mm) as toM.
+      pose proof (recvmChange st recvm_mm) as toM.
       pose proof (sendmChange dt markm_mm) as toM'.
       rewrite stEq in toM.
       rewrite dirEq in toM'.
       rewrite <- toM' in toM.
       assumption.
-      assert (noRecv: forall ti, ti < tm -> ~ proc mch p c a ti m) by
-          ( unfold not; intros ti ti_lt_tm proc'm;
-            pose proof (uniqProc2 procm proc'm) as ti_eq_tr; omega).
+      assert (noRecv: forall ti, ti < tm -> ~ recv mch p c a ti m) by
+          ( unfold not; intros ti ti_lt_tm recv'm;
+            pose proof (uniqRecv2 recvm recv'm) as ti_eq_tr; omega).
       pose proof (cross markm_mm markm noRecv) as noRecvFalse.
-      assert (ex2: exists tn, tn < ts /\ proc mch c p a tn mm) by
-          (destruct (classical (exists tn, tn < ts /\ proc mch c p a tn mm)) as [easy|easy'];
+      assert (ex2: exists tn, tn < ts /\ recv mch c p a tn mm) by
+          (destruct (classical (exists tn, tn < ts /\ recv mch c p a tn mm)) as [easy|easy'];
            [assumption |
             generalize noRecvFalse easy'; clear; firstorder]).
-      destruct ex2 as [tn [tn_lt_ts procmm]].
+      destruct ex2 as [tn [tn_lt_ts recvmm]].
       clear noRecvFalse.
-      assert (noPRecv: forall tk, tn < tk < ts -> forall mi, ~ proc mch c p a tk mi).
-      unfold not; intros tk [tn_lt_tk tk_lt_ts] mi procmi.
-      pose proof (procImpMark procmi) as [tl [tl_le_tk markmi]].
+      assert (noPRecv: forall tk, tn < tk < ts -> forall mi, ~ recv mch c p a tk mi).
+      unfold not; intros tk [tn_lt_tk tk_lt_ts] mi recvmi.
+      pose proof (recvImpMark recvmi) as [tl [tl_le_tk markmi]].
       assert (opts: tl = tm \/ tm < tl \/ tl < tm) by omega.
       destruct opts as [eq | [tm_lt_tl | tl_lt_tm]].
       rewrite eq in *.
       pose proof (uniqMark1 markm_mm markmi) as m_eq_mi.
       rewrite m_eq_mi in *.
-      pose proof (uniqProc2 procmm procmi) as sth.
+      pose proof (uniqRecv2 recvmm recvmi) as sth.
       omega.
       assert (tl_lt_tr: tl < tr) by omega.
       generalize notAfter tm_lt_tl tl_lt_tr markmi; clear; firstorder.
       pose proof @cRespFifo.
-      assert (notRecv: forall t4, t4 < tn -> ~ proc mch c p a t4 mi) by
-          (unfold not; intros t4 t4_lt_tn proc'mi;
-           pose proof (uniqProc2 procmi proc'mi) as t4_eq_tk; omega).
-      apply (cRespFifo markmi markm_mm procmm tl_lt_tm notRecv).
+      assert (notRecv: forall t4, t4 < tn -> ~ recv mch c p a t4 mi) by
+          (unfold not; intros t4 t4_lt_tn recv'mi;
+           pose proof (uniqRecv2 recvmi recv'mi) as t4_eq_tk; omega).
+      apply (cRespFifo markmi markm_mm recvmm tl_lt_tm notRecv).
       assert (noPSend: forall tk, tn < tk < ts -> forall mi, ~ mark mch p c a tk mi).
       unfold not; intros tk [tn_lt_tk tk_lt_ts] mi markmi.
-      pose proof (pRespFifo tk_lt_ts markmi markm procm) as [tl [tl_lt_tr procmi]].
-      pose proof (procImpMarkBefore procmi markmi) as tk_le_tl.
-      pose proof (procImpMarkBefore procmm markm_mm) as tm_le_tn.
+      pose proof (pRespFifo tk_lt_ts markmi markm recvm) as [tl [tl_lt_tr recvmi]].
+      pose proof (recvImpMarkBefore recvmi markmi) as tk_le_tl.
+      pose proof (recvImpMarkBefore recvmm markm_mm) as tm_le_tn.
       assert (tm_lt_tl: tm < tl) by omega.
-      generalize tm_lt_tl tl_lt_tr procmi notAfter; clear; firstorder.
+      generalize tm_lt_tl tl_lt_tr recvmi notAfter; clear; firstorder.
       assert (stEq: state c a (S tm) = state c a tr) by
           ( generalize (@noChange2 (state c) gt c p st a (S tm) tr tm_lt_tr) notAfter; clear; firstorder).
       assert (dirEq: dir p c a (S tn) = dir p c a ts) by
           ( generalize (@noChange2 (dir p c) lt p c dt a (S tn) ts tn_lt_ts) noPSend noPRecv; clear; firstorder).
-      pose proof (procmChange dt procmm) as toM.
+      pose proof (recvmChange dt recvmm) as toM.
       pose proof (sendmChange st markm_mm) as toM'.
       rewrite stEq in toM'.
       rewrite dirEq in toM.
       rewrite <- toM' in toM.
       auto.
-      pose proof (noCRespImpSameState procm markm) as good.
+      pose proof (noCRespImpSameState recvm markm) as good.
       generalize good notEx; clear; firstorder.
     Qed.
 
